ems/ModSemProof.v
@@ -9,7 +9,829 @@ Require Import STS Behavior.
 Require Import Any.
 Require Import Optics.
 
+Require Import Behavior.
+Require Import Relation_Definitions.
+
+(*** TODO: export these in Coqlib or Universe ***)
+Require Import Relation_Operators.
+Require Import RelationPairs.
+From ITree Require Import
+     Events.MapDefault
+     TranslateFacts.
+From ExtLib Require Import
+     Core.RelDec
+     Structures.Maps
+     Data.Map.FMapAList.
+Require Import Any.
+
+
 Set Implicit Arguments.
+
+
+
+Section SIM.
+  Let st_local: Type := (Any.t).
+
+  Variable world: Type.
+
+  Let W: Type := (Any.t) * (Any.t).
+  Variable wf : world -> W -> Prop.
+  Variable le: relation world.
+
+
+  Inductive _sim_itree (sim_itree: forall (R_src R_tgt: Type) (RR: st_local -> st_local -> R_src -> R_tgt -> Prop), bool -> bool -> world -> st_local * itree Es R_src -> st_local * itree Es R_tgt -> Prop)
+          {R_src R_tgt} (RR: st_local -> st_local -> R_src -> R_tgt -> Prop)
+    : bool -> bool -> world -> st_local * itree Es R_src -> st_local * itree Es R_tgt -> Prop :=
+  | sim_itree_ret
+      i_src0 i_tgt0 w0 st_src0 st_tgt0
+      v_src v_tgt
+      (RET: RR st_src0 st_tgt0 v_src v_tgt)
+    :
+      _sim_itree sim_itree RR i_src0 i_tgt0 w0 (st_src0, Ret v_src) (st_tgt0, Ret v_tgt)
+
+  | sim_itree_call
+      i_src0 i_tgt0 w w0 st_src0 st_tgt0
+      fn varg k_src k_tgt
+      (WF: wf w0 (st_src0, st_tgt0))
+      (K: forall w1 vret st_src1 st_tgt1 (WLE: le w0 w1) (WF: wf w1 (st_src1, st_tgt1)),
+          sim_itree _ _ RR false false w (st_src1, k_src vret) (st_tgt1, k_tgt vret))
+    :
+      _sim_itree sim_itree RR i_src0 i_tgt0 w (st_src0, trigger (Call fn varg) >>= k_src)
+                 (st_tgt0, trigger (Call fn varg) >>= k_tgt)
+
+  | sim_itree_syscall
+      i_src0 i_tgt0 w0 st_src0 st_tgt0
+      fn varg rvs k_src k_tgt
+      (K: forall vret,
+          sim_itree _ _ RR true true w0 (st_src0, k_src vret) (st_tgt0, k_tgt vret))
+    :
+      _sim_itree sim_itree RR i_src0 i_tgt0 w0 (st_src0, trigger (Syscall fn varg rvs) >>= k_src)
+                 (st_tgt0, trigger (Syscall fn varg rvs) >>= k_tgt)
+
+  | sim_itree_tau_src
+      i_src0 i_tgt0 w0 (st_src0: st_local) (st_tgt0: st_local)
+      i_src i_tgt
+      (K: _sim_itree sim_itree RR true i_tgt0 w0 (st_src0, i_src) (st_tgt0, i_tgt))
+    :
+      _sim_itree sim_itree RR i_src0 i_tgt0 w0 (st_src0, tau;; i_src) (st_tgt0, i_tgt)
+
+  | sim_itree_tau_tgt
+      i_src0 i_tgt0 w0 (st_src0: st_local) (st_tgt0: st_local)
+      i_src i_tgt
+      (K: _sim_itree sim_itree RR i_src0 true w0 (st_src0, i_src) (st_tgt0, i_tgt))
+    :
+      _sim_itree sim_itree RR i_src0 i_tgt0 w0 (st_src0, i_src) (st_tgt0, tau;; i_tgt)
+
+  | sim_itree_choose_src
+      i_src0 i_tgt0 w0 (st_src0: st_local) (st_tgt0: st_local)
+      X k_src i_tgt
+      (K: exists (x: X), _sim_itree sim_itree RR true i_tgt0 w0 (st_src0, k_src x) (st_tgt0, i_tgt))
+    :
+      _sim_itree sim_itree RR i_src0 i_tgt0 w0 (st_src0, trigger (Choose X) >>= k_src)
+                 (st_tgt0, i_tgt)
+
+  | sim_itree_choose_tgt
+      i_src0 i_tgt0 w0 (st_src0: st_local) (st_tgt0: st_local)
+      X i_src k_tgt
+      (K: forall (x: X), _sim_itree sim_itree RR i_src0 true w0 (st_src0, i_src) (st_tgt0, k_tgt x))
+    :
+      _sim_itree sim_itree RR i_src0 i_tgt0 w0 (st_src0, i_src)
+                 (st_tgt0, trigger (Choose X) >>= k_tgt)
+
+  | sim_itree_take_src
+      i_src0 i_tgt0 w0 (st_src0: st_local) (st_tgt0: st_local)
+      X k_src i_tgt
+      (K: forall (x: X), _sim_itree sim_itree RR true i_tgt0 w0 (st_src0, k_src x) (st_tgt0, i_tgt))
+    :
+      _sim_itree sim_itree RR i_src0 i_tgt0 w0 (st_src0, trigger (Take X) >>= k_src)
+                 (st_tgt0, i_tgt)
+
+  | sim_itree_take_tgt
+      i_src0 i_tgt0 w0 (st_src0: st_local) (st_tgt0: st_local)
+      X i_src k_tgt
+      (K: exists (x: X), _sim_itree sim_itree RR i_src0 true w0 (st_src0, i_src) (st_tgt0, k_tgt x))
+    :
+      _sim_itree sim_itree RR i_src0 i_tgt0 w0 (st_src0, i_src)
+                 (st_tgt0, trigger (Take X) >>= k_tgt)
+
+  | sim_itree_supdate_src
+      i_src0 i_tgt0 w0 (st_src0: st_local) (st_tgt0: st_local)
+      X k_src i_tgt
+      (run: st_local -> st_local * X )
+      (K: _sim_itree sim_itree RR true i_tgt0 w0 (fst (run st_src0), k_src (snd (run st_src0))) (st_tgt0, i_tgt))
+    :
+      _sim_itree sim_itree RR i_src0 i_tgt0 w0 (st_src0, trigger (SUpdate run) >>= k_src) (st_tgt0, i_tgt)  
+
+  | sim_itree_supdate_tgt
+      i_src0 i_tgt0 w0 (st_src0: st_local) (st_tgt0: st_local)
+      X i_src k_tgt
+      (run: st_local -> st_local * X )
+      (K: _sim_itree sim_itree RR i_src0 true w0 (st_src0, i_src) (fst (run st_tgt0), k_tgt (snd (run st_tgt0))))
+    :
+      _sim_itree sim_itree RR i_src0 i_tgt0 w0 (st_src0, i_src) (st_tgt0, trigger (SUpdate run) >>= k_tgt)
+
+  | sim_itree_progress
+      i_src0 i_tgt0 w0 (st_src0: st_local) (st_tgt0: st_local) i_src i_tgt
+      (SIM: sim_itree _ _ RR false false w0 (st_src0, i_src) (st_tgt0, i_tgt))
+      (SRC: i_src0 = true)
+      (TGT: i_tgt0 = true)
+    :
+      _sim_itree sim_itree RR true true w0 (st_src0, i_src) (st_tgt0, i_tgt)
+  .
+
+  Definition lift_rel {R_src R_tgt} (w0: world) (RR: R_src -> R_tgt -> Prop)
+             (st_src0: st_local) (st_tgt0: st_local) (ret_src ret_tgt: Any.t) :=
+    exists w1 : world,
+      (<<WLE: le w0 w1 >> /\ <<WF: wf w1 (st_src0, st_tgt0) >> /\ <<RET: ret_src = ret_tgt >>).
+
+  Lemma _sim_itree_ind2 (sim_itree: forall (R_src R_tgt: Type) 
+                                    (RR: st_local -> st_local -> R_src -> R_tgt -> Prop), bool -> bool -> world -> st_local * itree Es R_src -> st_local * itree Es R_tgt -> Prop)
+        {R_src R_tgt} (RR: st_local -> st_local -> R_src -> R_tgt -> Prop)
+        (P: bool -> bool -> world -> st_local * itree Es R_src -> st_local * itree Es R_tgt -> Prop)
+        (RET: forall
+            i_src0 i_tgt0 w0 st_src0 st_tgt0
+            v_src v_tgt
+            (RET: RR st_src0 st_tgt0 v_src v_tgt),
+            P i_src0 i_tgt0 w0 (st_src0, Ret v_src) (st_tgt0, Ret v_tgt))
+        (CALL: forall
+            i_src0 i_tgt0 w w0 st_src0 st_tgt0
+            fn varg k_src k_tgt
+            (WF: wf w0 (st_src0, st_tgt0))
+            (K: forall w1 vret st_src1 st_tgt1 (WLE: le w0 w1) (WF: wf w1 (st_src1, st_tgt1)),
+                sim_itree _ _ RR false false w (st_src1, k_src vret) (st_tgt1, k_tgt vret)),
+            P i_src0 i_tgt0 w (st_src0, trigger (Call fn varg) >>= k_src)
+              (st_tgt0, trigger (Call fn varg) >>= k_tgt))
+        (SYSCALL: forall
+            i_src0 i_tgt0 w0 (st_src0: st_local) (st_tgt0: st_local)
+            fn varg rvs k_src k_tgt
+            (K: forall vret,
+                sim_itree _ _ RR true true w0 (st_src0, k_src vret) (st_tgt0, k_tgt vret)),
+            P i_src0 i_tgt0 w0 (st_src0, trigger (Syscall fn varg rvs) >>= k_src)
+              (st_tgt0, trigger (Syscall fn varg rvs) >>= k_tgt))
+        (TAUSRC: forall
+            i_src0 i_tgt0 w0 (st_src0: st_local) (st_tgt0: st_local)
+            i_src i_tgt
+            (K: _sim_itree sim_itree RR true i_tgt0 w0 (st_src0, i_src) (st_tgt0, i_tgt))
+            (IH: P true i_tgt0 w0 (st_src0, i_src) (st_tgt0, i_tgt)),
+            P i_src0 i_tgt0 w0 (st_src0, tau;; i_src) (st_tgt0, i_tgt))
+        (TAUTGT: forall
+            i_src0 i_tgt0 w0 (st_src0: st_local) (st_tgt0: st_local)
+            i_src i_tgt
+            (K: _sim_itree sim_itree RR i_src0 true w0 (st_src0, i_src) (st_tgt0, i_tgt))
+            (IH: P i_src0 true w0 (st_src0, i_src) (st_tgt0, i_tgt)),
+            P i_src0 i_tgt0 w0 (st_src0, i_src) (st_tgt0, tau;; i_tgt))
+        (CHOOSESRC: forall
+            i_src0 i_tgt0 w0 (st_src0: st_local) (st_tgt0: st_local)
+            X k_src i_tgt
+            (K: exists (x: X), <<SIM: _sim_itree sim_itree RR true i_tgt0 w0 (st_src0, k_src x) (st_tgt0, i_tgt)>> /\ <<IH: P true i_tgt0 w0 (st_src0, k_src x) (st_tgt0, i_tgt)>>),
+            P i_src0 i_tgt0 w0 (st_src0, trigger (Choose X) >>= k_src)
+              (st_tgt0, i_tgt))
+        (CHOOSETGT: forall
+            i_src0 i_tgt0 w0 (st_src0: st_local) (st_tgt0: st_local)
+            X i_src k_tgt
+            (K: forall (x: X), <<SIMH: _sim_itree sim_itree RR i_src0 true w0 (st_src0, i_src) (st_tgt0, k_tgt x)>> /\ <<IH: P i_src0 true w0 (st_src0, i_src) (st_tgt0, k_tgt x)>>),
+            P i_src0 i_tgt0 w0 (st_src0, i_src)
+              (st_tgt0, trigger (Choose X) >>= k_tgt))
+        (TAKESRC: forall
+            i_src0 i_tgt0 w0 (st_src0: st_local) (st_tgt0: st_local)
+            X k_src i_tgt
+            (K: forall (x: X), <<SIM: _sim_itree sim_itree RR true i_tgt0 w0 (st_src0, k_src x) (st_tgt0, i_tgt)>> /\ <<IH: P true i_tgt0 w0 (st_src0, k_src x) (st_tgt0, i_tgt)>>),
+            P i_src0 i_tgt0 w0 (st_src0, trigger (Take X) >>= k_src)
+              (st_tgt0, i_tgt))
+        (TAKETGT: forall
+            i_src0 i_tgt0 w0 (st_src0: st_local) (st_tgt0: st_local)
+            X i_src k_tgt
+            (K: exists (x: X), <<SIM:_sim_itree sim_itree RR i_src0 true w0 (st_src0, i_src) (st_tgt0, k_tgt x)>> /\ <<IH: P i_src0 true w0 (st_src0, i_src) (st_tgt0, k_tgt x)>>),
+            P i_src0 i_tgt0 w0 (st_src0, i_src)
+              (st_tgt0, trigger (Take X) >>= k_tgt))
+        (SUPDATESRC: forall
+            i_src0 i_tgt0 w0 (st_src0: st_local) (st_tgt0: st_local)
+            X k_src i_tgt
+            (run: st_local -> st_local * X )
+            (K: _sim_itree sim_itree RR true i_tgt0 w0 (fst (run st_src0), k_src (snd (run st_src0))) (st_tgt0, i_tgt))
+            (IH: P true i_tgt0 w0 (fst (run st_src0), k_src (snd (run st_src0))) (st_tgt0, i_tgt)),
+            P i_src0 i_tgt0 w0 (st_src0, trigger (SUpdate run) >>= k_src) (st_tgt0, i_tgt))
+        (SUPDATETGT: forall
+            i_src0 i_tgt0 w0 (st_src0: st_local) (st_tgt0: st_local)
+            X i_src k_tgt
+            (run: st_local -> st_local * X )
+            (K: _sim_itree sim_itree RR i_src0 true w0 (st_src0, i_src) (fst (run st_tgt0), k_tgt (snd (run st_tgt0))))
+            (IH: P i_src0 true w0 (st_src0, i_src) (fst (run st_tgt0), k_tgt (snd (run st_tgt0)))),
+            P i_src0 i_tgt0 w0 (st_src0, i_src) (st_tgt0, trigger (SUpdate run) >>= k_tgt))
+        (PROGRESS: forall
+            i_src0 i_tgt0 w0 (st_src0: st_local) (st_tgt0: st_local) i_src i_tgt
+            (SIM: sim_itree _ _ RR false false w0 (st_src0, i_src) (st_tgt0, i_tgt))
+            (SRC: i_src0 = true)
+            (TGT: i_tgt0 = true),
+            P true true w0 (st_src0, i_src) (st_tgt0, i_tgt))
+    :
+      forall i_src0 i_tgt0 w0 st_src st_tgt
+             (SIM: _sim_itree sim_itree RR i_src0 i_tgt0 w0 st_src st_tgt),
+        P i_src0 i_tgt0 w0 st_src st_tgt.
+  Proof.
+    fix IH 6. i. inv SIM.
+    { eapply RET; eauto. }
+    { eapply CALL; eauto. }
+    { eapply SYSCALL; eauto. }
+    { eapply TAUSRC; eauto. }
+    { eapply TAUTGT; eauto. }
+    { eapply CHOOSESRC; eauto. des. esplits; eauto. }
+    { eapply CHOOSETGT; eauto. }
+    { eapply TAKESRC; eauto. }
+    { eapply TAKETGT; eauto. des. esplits; eauto. }
+    { eapply SUPDATESRC; eauto. }
+    { eapply SUPDATETGT; eauto. }
+    { eapply PROGRESS; eauto. }
+
+  Qed.
+
+  Definition sim_itree o_src o_tgt w0 : relation _ :=
+    paco8 _sim_itree bot8 _ _ (lift_rel w0 (@eq Any.t)) o_src o_tgt w0.
+
+  Lemma sim_itree_mon: monotone8 _sim_itree.
+  Proof.
+    ii. induction IN using _sim_itree_ind2; try (by des; econs; ss; et).
+    - econs; ss; et. ii. exploit K; et. i; des. esplits; et.
+    - econs; ss; et. ii. exploit K; et. i; des. esplits; et.
+  Qed.
+
+  Hint Constructors _sim_itree.
+  Hint Unfold sim_itree.
+  Hint Resolve sim_itree_mon: paco.
+  Hint Resolve cpn8_wcompat: paco.
+
+  Lemma sim_itree_ind
+        R_src R_tgt (RR: st_local -> st_local -> R_src -> R_tgt -> Prop) 
+        (P: bool -> bool -> world -> st_local * itree Es R_src -> st_local * itree Es R_tgt -> Prop)
+        (RET: forall
+            i_src0 i_tgt0 w0 st_src0 st_tgt0
+            v_src v_tgt
+            (RET: RR st_src0 st_tgt0 v_src v_tgt),
+            P i_src0 i_tgt0 w0 (st_src0, Ret v_src) (st_tgt0, Ret v_tgt))
+        (CALL: forall
+            i_src0 i_tgt0 w w0 st_src0 st_tgt0
+            fn varg k_src k_tgt
+            (WF: wf w0 (st_src0, st_tgt0))
+            (K: forall w1 vret st_src1 st_tgt1 (WLE: le w0 w1) (WF: wf w1 (st_src1, st_tgt1)),
+                paco8 _sim_itree bot8 _ _ RR false false w (st_src1, k_src vret) (st_tgt1, k_tgt vret)),
+            P i_src0 i_tgt0 w (st_src0, trigger (Call fn varg) >>= k_src)
+              (st_tgt0, trigger (Call fn varg) >>= k_tgt))
+        (SYSCALL: forall
+            i_src0 i_tgt0 w0 (st_src0: st_local) (st_tgt0: st_local)
+            fn varg rvs k_src k_tgt
+            (K: forall vret,
+                paco8 _sim_itree bot8 _ _ RR true true w0 (st_src0, k_src vret) (st_tgt0, k_tgt vret)),
+            P i_src0 i_tgt0 w0 (st_src0, trigger (Syscall fn varg rvs) >>= k_src)
+              (st_tgt0, trigger (Syscall fn varg rvs) >>= k_tgt))
+        (TAUSRC: forall
+            i_src0 i_tgt0 w0 (st_src0: st_local) (st_tgt0: st_local)
+            i_src i_tgt
+            (K: paco8 _sim_itree bot8 _ _ RR true i_tgt0 w0 (st_src0, i_src) (st_tgt0, i_tgt))
+            (IH: P true i_tgt0 w0 (st_src0, i_src) (st_tgt0, i_tgt)),
+            P i_src0 i_tgt0 w0 (st_src0, tau;; i_src) (st_tgt0, i_tgt))
+        (TAUTGT: forall
+            i_src0 i_tgt0 w0 (st_src0: st_local) (st_tgt0: st_local)
+            i_src i_tgt
+            (K: paco8 _sim_itree bot8 _ _ RR i_src0 true w0 (st_src0, i_src) (st_tgt0, i_tgt))
+            (IH: P i_src0 true w0 (st_src0, i_src) (st_tgt0, i_tgt)),
+            P i_src0 i_tgt0 w0 (st_src0, i_src) (st_tgt0, tau;; i_tgt))            
+        (CHOOSESRC: forall
+            i_src0 i_tgt0 w0 (st_src0: st_local) (st_tgt0: st_local)
+            X k_src i_tgt
+            (K: exists (x: X), <<SIM: paco8 _sim_itree bot8 _ _ RR true i_tgt0 w0 (st_src0, k_src x) (st_tgt0, i_tgt)>> /\ <<IH: P true i_tgt0 w0 (st_src0, k_src x) (st_tgt0, i_tgt)>>),
+            P i_src0 i_tgt0 w0 (st_src0, trigger (Choose X) >>= k_src)
+              (st_tgt0, i_tgt))
+        (CHOOSETGT: forall
+            i_src0 i_tgt0 w0 (st_src0: st_local) (st_tgt0: st_local)
+            X i_src k_tgt
+            (K: forall (x: X), <<SIMH: paco8 _sim_itree bot8 _ _ RR i_src0 true w0 (st_src0, i_src) (st_tgt0, k_tgt x)>> /\ <<IH: P i_src0 true w0 (st_src0, i_src) (st_tgt0, k_tgt x)>>),
+            P i_src0 i_tgt0 w0 (st_src0, i_src)
+              (st_tgt0, trigger (Choose X) >>= k_tgt))
+        (TAKESRC: forall
+            i_src0 i_tgt0 w0 (st_src0: st_local) (st_tgt0: st_local)
+            X k_src i_tgt
+            (K: forall (x: X), <<SIM: paco8 _sim_itree bot8 _ _ RR true i_tgt0 w0 (st_src0, k_src x) (st_tgt0, i_tgt)>> /\ <<IH: P true i_tgt0 w0 (st_src0, k_src x) (st_tgt0, i_tgt)>>),
+            P i_src0 i_tgt0 w0 (st_src0, trigger (Take X) >>= k_src)
+              (st_tgt0, i_tgt))
+        (TAKETGT: forall
+            i_src0 i_tgt0 w0 (st_src0: st_local) (st_tgt0: st_local)
+            X i_src k_tgt
+            (K: exists (x: X), <<SIM:paco8 _sim_itree bot8 _ _ RR i_src0 true w0 (st_src0, i_src) (st_tgt0, k_tgt x)>> /\ <<IH: P i_src0 true w0 (st_src0, i_src) (st_tgt0, k_tgt x)>>),
+            P i_src0 i_tgt0 w0 (st_src0, i_src)
+              (st_tgt0, trigger (Take X) >>= k_tgt))
+        (SUPDATESRC: forall
+            i_src0 i_tgt0 w0 (st_src0: st_local) (st_tgt0: st_local)
+            X k_src i_tgt
+            (run: st_local -> st_local * X )
+            (K: paco8 _sim_itree bot8 _ _ RR true i_tgt0 w0 (fst (run st_src0), k_src (snd (run st_src0))) (st_tgt0, i_tgt))
+            (IH: P true i_tgt0 w0 (fst (run st_src0), k_src (snd (run st_src0))) (st_tgt0, i_tgt)),
+            P i_src0 i_tgt0 w0 (st_src0, trigger (SUpdate run) >>= k_src) (st_tgt0, i_tgt))
+        (SUPDATETGT: forall
+            i_src0 i_tgt0 w0 (st_src0: st_local) (st_tgt0: st_local)
+            X i_src k_tgt
+            (run: st_local -> st_local * X )
+            (K: paco8 _sim_itree bot8 _ _ RR i_src0 true w0 (st_src0, i_src) (fst (run st_tgt0), k_tgt (snd (run st_tgt0))))
+            (IH:  P i_src0 true w0 (st_src0, i_src) (fst (run st_tgt0), k_tgt (snd (run st_tgt0)))),
+
+            P i_src0 i_tgt0 w0 (st_src0, i_src) (st_tgt0, trigger (SUpdate run) >>= k_tgt))       
+        (PROGRESS: forall
+            i_src0 i_tgt0 w0 (st_src0: st_local) (st_tgt0: st_local)
+            i_src i_tgt
+            (SIM: paco8 _sim_itree bot8 _ _ RR false false w0 (st_src0, i_src) (st_tgt0, i_tgt))
+            (SRC: i_src0 = true)
+            (TGT: i_tgt0 = true),
+            P true true w0 (st_src0, i_src) (st_tgt0, i_tgt))
+    :
+      forall i_src0 i_tgt0 w0 st_src st_tgt
+             (SIM: paco8 _sim_itree bot8 _ _ RR i_src0 i_tgt0 w0 st_src st_tgt),
+        P i_src0 i_tgt0 w0 st_src st_tgt.
+  Proof.
+    i. punfold SIM. induction SIM using _sim_itree_ind2.
+    { eapply RET; eauto. }
+    { eapply CALL; eauto. i. exploit K; eauto. i. pclearbot. eauto. }
+    { eapply SYSCALL; eauto. i. exploit K; eauto. i. pclearbot. eauto. }
+    { eapply TAUSRC; eauto. }
+    { eapply TAUTGT; eauto. }
+    { eapply CHOOSESRC; eauto. des. esplits; eauto. }
+    { eapply CHOOSETGT; eauto. i. exploit K; eauto. i. des.
+    pclearbot. esplits; eauto. }
+    { eapply TAKESRC; eauto. i. exploit K; eauto. i. des.
+      pclearbot. esplits; eauto. }
+    { eapply TAKETGT; eauto. des. esplits; eauto. }
+    { eapply SUPDATESRC; eauto. }
+    { eapply SUPDATETGT; eauto. }
+    { eapply PROGRESS; eauto. pclearbot. auto. }
+
+  Qed.
+
+  Variant sim_itree_indC (sim_itree: forall (R_src R_tgt: Type) (RR: st_local -> st_local -> R_src -> R_tgt -> Prop), bool -> bool -> world -> st_local * itree Es R_src -> st_local * itree Es R_tgt -> Prop)
+          {R_src R_tgt} (RR: st_local -> st_local -> R_src -> R_tgt -> Prop)
+    : bool -> bool -> world -> st_local * itree Es R_src -> st_local * itree Es R_tgt -> Prop :=
+  | sim_itree_indC_ret
+      i_src0 i_tgt0 w0 st_src0 st_tgt0
+      v_src v_tgt
+      (RET: RR st_src0 st_tgt0 v_src v_tgt)
+    :
+      sim_itree_indC  sim_itree RR i_src0 i_tgt0 w0 (st_src0, Ret v_src) (st_tgt0, Ret v_tgt)
+  | sim_itree_indC_call
+      i_src0 i_tgt0 w w0 st_src0 st_tgt0
+      fn varg k_src k_tgt
+      (WF: wf w0 (st_src0, st_tgt0))
+      (K: forall w1 vret st_src1 st_tgt1 (WLE: le w0 w1) (WF: wf w1 (st_src1, st_tgt1)),
+          sim_itree _ _ RR false false w (st_src1, k_src vret) (st_tgt1, k_tgt vret))
+    :
+      sim_itree_indC  sim_itree RR i_src0 i_tgt0 w (st_src0, trigger (Call fn varg) >>= k_src)
+                     (st_tgt0, trigger (Call fn varg) >>= k_tgt)
+  | sim_itree_indC_syscall
+      i_src0 i_tgt0 w0 (st_src0: st_local) (st_tgt0: st_local)
+      fn varg rvs k_src k_tgt
+      (K: forall vret,
+          sim_itree _ _ RR true true w0 (st_src0, k_src vret) (st_tgt0, k_tgt vret))
+    :
+      sim_itree_indC  sim_itree RR i_src0 i_tgt0 w0 (st_src0, trigger (Syscall fn varg rvs) >>= k_src)
+                     (st_tgt0, trigger (Syscall fn varg rvs) >>= k_tgt)
+
+  | sim_itree_indC_tau_src
+      i_src0 i_tgt0 w0 (st_src0: st_local) (st_tgt0: st_local)
+      i_src i_tgt
+      (K: sim_itree _ _ RR true i_tgt0 w0 (st_src0, i_src) (st_tgt0, i_tgt))
+    :
+      sim_itree_indC  sim_itree RR i_src0 i_tgt0 w0 (st_src0, tau;; i_src) (st_tgt0, i_tgt)
+
+  | sim_itree_indC_tau_tgt
+      i_src0 i_tgt0 w0 (st_src0: st_local) (st_tgt0: st_local)
+      i_src i_tgt
+      (K: sim_itree _ _ RR i_src0 true w0 (st_src0, i_src) (st_tgt0, i_tgt))
+    :
+      sim_itree_indC  sim_itree RR i_src0 i_tgt0 w0 (st_src0, i_src) (st_tgt0, tau;; i_tgt)
+
+  | sim_itree_indC_choose_src
+      i_src0 i_tgt0 w0 (st_src0: st_local) (st_tgt0: st_local)
+      X k_src i_tgt
+      (K: exists (x: X), sim_itree _ _ RR true i_tgt0 w0 (st_src0, k_src x) (st_tgt0, i_tgt))
+    :
+      sim_itree_indC  sim_itree RR i_src0 i_tgt0 w0 (st_src0, trigger (Choose X) >>= k_src)
+                     (st_tgt0, i_tgt)
+  | sim_itree_indC_choose_tgt
+      i_src0 i_tgt0 w0 (st_src0: st_local) (st_tgt0: st_local)
+      X i_src k_tgt
+      (K: forall (x: X), sim_itree _ _ RR i_src0 true w0 (st_src0, i_src) (st_tgt0, k_tgt x))
+    :
+      sim_itree_indC  sim_itree RR i_src0 i_tgt0 w0 (st_src0, i_src)
+                     (st_tgt0, trigger (Choose X) >>= k_tgt)
+
+  | sim_itree_indC_take_src
+      i_src0 i_tgt0 w0 (st_src0: st_local) (st_tgt0: st_local)
+      X k_src i_tgt
+      (K: forall (x: X), sim_itree _ _ RR true i_tgt0 w0 (st_src0, k_src x) (st_tgt0, i_tgt))
+    :
+      sim_itree_indC  sim_itree RR i_src0 i_tgt0 w0 (st_src0, trigger (Take X) >>= k_src)
+                     (st_tgt0, i_tgt)
+  | sim_itree_indC_take_tgt
+      i_src0 i_tgt0 w0 (st_src0: st_local) (st_tgt0: st_local)
+      X i_src k_tgt
+      (K: exists (x: X), sim_itree _ _ RR i_src0 true w0 (st_src0, i_src) (st_tgt0, k_tgt x))
+    :
+      sim_itree_indC  sim_itree RR i_src0 i_tgt0 w0 (st_src0, i_src)
+                     (st_tgt0, trigger (Take X) >>= k_tgt)
+  
+  | sim_itree_indC_supdate_src
+      i_src0 i_tgt0 w0 (st_src0: st_local) (st_tgt0: st_local)
+      X k_src i_tgt
+      (run: st_local -> st_local * X )
+      (K: sim_itree _ _ RR true i_tgt0 w0 (fst (run st_src0), k_src (snd (run st_src0))) (st_tgt0, i_tgt))
+    :
+      sim_itree_indC  sim_itree RR i_src0 i_tgt0 w0 (st_src0, trigger (SUpdate run) >>= k_src) (st_tgt0, i_tgt)
+
+  | sim_itree_indC_supdate_tgt
+      i_src0 i_tgt0 w0 (st_src0: st_local) (st_tgt0: st_local)
+      X i_src k_tgt
+      (run: st_local -> st_local * X )
+      (K: sim_itree _ _ RR i_src0 true w0 (st_src0, i_src) (fst (run st_tgt0), k_tgt (snd (run st_tgt0))))
+    :
+      sim_itree_indC  sim_itree RR i_src0 i_tgt0 w0 (st_src0, i_src) (st_tgt0, trigger (SUpdate run) >>= k_tgt)
+  .
+
+  Lemma sim_itree_indC_mon: monotone8 sim_itree_indC.
+  Proof.
+    ii. inv IN; try (by des; econs; ss; et).
+  Qed.
+  Hint Resolve sim_itree_indC_mon: paco.
+
+  Lemma sim_itree_indC_spec:
+    sim_itree_indC <9= gupaco8 (_sim_itree) (cpn8 _sim_itree).
+  Proof.
+    eapply wrespect8_uclo; eauto with paco.
+    econs; eauto with paco. i. inv PR.
+    { econs 1; eauto. }
+    { econs 2; eauto. i. exploit K; eauto. i. des.
+      esplits; eauto. eapply rclo8_base. eauto. }
+    { econs 3; eauto. i. eapply rclo8_base. eauto. }
+    { econs 4; eauto. eapply sim_itree_mon; eauto. i. eapply rclo8_base. eauto. }
+    { econs 5; eauto. eapply sim_itree_mon; eauto. i. eapply rclo8_base. eauto. }
+    { econs 6; eauto. des. esplits; eauto. eapply sim_itree_mon; eauto. i. eapply rclo8_base. eauto. }
+    { econs 7; eauto. i. eapply sim_itree_mon; eauto. i. eapply rclo8_base. eauto. }
+    { econs 8; eauto. i. eapply sim_itree_mon; eauto. i. eapply rclo8_base. eauto. }
+    { econs 9; eauto. des. esplits; eauto. eapply sim_itree_mon; eauto. i. eapply rclo8_base. eauto. }
+    { econs 10; eauto. des. esplits; eauto. eapply sim_itree_mon; eauto. i. eapply rclo8_base. eauto.  }
+    { econs 11; eauto. des. esplits; eauto.  eapply sim_itree_mon; eauto. i. eapply rclo8_base. eauto.  }
+  Qed.
+
+  Variant sim_itreeC (r g: forall (R_src R_tgt: Type) (RR: st_local -> st_local -> R_src -> R_tgt -> Prop), bool -> bool -> world -> st_local * itree Es R_src -> st_local * itree Es R_tgt -> Prop)
+          {R_src R_tgt} (RR: st_local -> st_local -> R_src -> R_tgt -> Prop)
+    : bool -> bool -> world -> st_local * itree Es R_src -> st_local * itree Es R_tgt -> Prop :=
+  | sim_itreeC_ret
+      i_src0 i_tgt0 w0 st_src0 st_tgt0
+      v_src v_tgt
+      (RET: RR st_src0 st_tgt0 v_src v_tgt)
+    :
+      sim_itreeC r g RR i_src0 i_tgt0 w0 (st_src0, Ret v_src) (st_tgt0, Ret v_tgt)
+  | sim_itreeC_call
+      i_src0 i_tgt0 w w0 st_src0 st_tgt0
+      fn varg k_src k_tgt
+      (WF: wf w0 (st_src0, st_tgt0))
+      (K: forall w1 vret st_src1 st_tgt1 (WLE: le w0 w1) (WF: wf w1 (st_src1, st_tgt1)),
+          g _ _ RR false false w (st_src1, k_src vret) (st_tgt1, k_tgt vret))
+    :
+      sim_itreeC r g RR i_src0 i_tgt0 w (st_src0, trigger (Call fn varg) >>= k_src)
+                 (st_tgt0, trigger (Call fn varg) >>= k_tgt)
+  | sim_itreeC_syscall
+      i_src0 i_tgt0 w0 (st_src0: st_local) (st_tgt0: st_local)
+      fn varg rvs k_src k_tgt
+      (K: forall vret,
+          g _ _ RR true true w0 (st_src0, k_src vret) (st_tgt0, k_tgt vret))
+    :
+      sim_itreeC r g RR i_src0 i_tgt0 w0 (st_src0, trigger (Syscall fn varg rvs) >>= k_src)
+                 (st_tgt0, trigger (Syscall fn varg rvs) >>= k_tgt)
+
+  | sim_itreeC_tau_src
+      i_src0 i_tgt0 w0 (st_src0: st_local) (st_tgt0: st_local)
+      i_src i_tgt
+      (K: r _ _ RR true i_tgt0 w0 (st_src0, i_src) (st_tgt0, i_tgt))
+    :
+      sim_itreeC r g RR i_src0 i_tgt0 w0 (st_src0, tau;; i_src) (st_tgt0, i_tgt)
+
+  | sim_itreeC_tau_tgt
+      i_src0 i_tgt0 w0 (st_src0: st_local) (st_tgt0: st_local)
+      i_src i_tgt
+      (K: r _ _ RR i_src0 true w0 (st_src0, i_src) (st_tgt0, i_tgt))
+    :
+      sim_itreeC r g RR i_src0 i_tgt0 w0 (st_src0, i_src) (st_tgt0, tau;; i_tgt)
+
+
+  | sim_itreeC_choose_src
+      i_src0 i_tgt0 w0 (st_src0: st_local) (st_tgt0: st_local)
+      X k_src i_tgt
+      (K: exists (x: X), r _ _ RR true i_tgt0 w0 (st_src0, k_src x) (st_tgt0, i_tgt))
+    :
+      sim_itreeC r g RR i_src0 i_tgt0 w0 (st_src0, trigger (Choose X) >>= k_src)
+                 (st_tgt0, i_tgt)
+  | sim_itreeC_choose_tgt
+      i_src0 i_tgt0 w0 (st_src0: st_local) (st_tgt0: st_local)
+      X i_src k_tgt
+      (K: forall (x: X), r _ _ RR i_src0 true w0 (st_src0, i_src) (st_tgt0, k_tgt x))
+    :
+      sim_itreeC r g RR i_src0 i_tgt0 w0 (st_src0, i_src)
+                 (st_tgt0, trigger (Choose X) >>= k_tgt)
+  | sim_itreeC_take_src
+      i_src0 i_tgt0 w0 (st_src0: st_local) (st_tgt0: st_local)
+      X k_src i_tgt
+      (K: forall (x: X), r _ _ RR true i_tgt0 w0 (st_src0, k_src x) (st_tgt0, i_tgt))
+    :
+      sim_itreeC r g RR i_src0 i_tgt0 w0 (st_src0, trigger (Take X) >>= k_src)
+                 (st_tgt0, i_tgt)
+  | sim_itreeC_take_tgt
+      i_src0 i_tgt0 w0 (st_src0: st_local) (st_tgt0: st_local)
+      X i_src k_tgt
+      (K: exists (x: X), r _ _ RR i_src0 true w0 (st_src0, i_src) (st_tgt0, k_tgt x))
+    :
+      sim_itreeC r g RR i_src0 i_tgt0 w0 (st_src0, i_src)
+                 (st_tgt0, trigger (Take X) >>= k_tgt)
+  | sim_itreeC_supdate_src
+      i_src0 i_tgt0 w0 (st_src0: st_local) (st_tgt0: st_local)
+      X k_src i_tgt
+      (run: st_local -> st_local * X )
+      (K: r _ _ RR true i_tgt0 w0 (fst (run st_src0), k_src (snd (run st_src0))) (st_tgt0, i_tgt))
+    :
+      sim_itreeC r g RR i_src0 i_tgt0 w0 (st_src0, trigger (SUpdate run) >>= k_src) (st_tgt0, i_tgt)
+
+  | sim_itreeC_supdate_tgt
+      i_src0 i_tgt0 w0 (st_src0: st_local) (st_tgt0: st_local)
+      X i_src k_tgt
+      (run: st_local -> st_local * X )
+      (K: r _ _ RR i_src0 true w0 (st_src0, i_src) (fst (run st_tgt0), k_tgt (snd (run st_tgt0))))
+    :
+      sim_itreeC r g RR i_src0 i_tgt0 w0 (st_src0, i_src) (st_tgt0, trigger (SUpdate run) >>= k_tgt)
+
+  .
+
+  Lemma sim_itreeC_spec_aux:
+    sim_itreeC <10= gpaco8 (_sim_itree) (cpn8 _sim_itree).
+  Proof.
+    i. inv PR.
+    { gstep. econs 1; eauto. }
+    { gstep. econs 2; eauto. i. gbase. eauto. }
+    { gstep. econs 3; eauto. i. gbase. eauto. }
+    { guclo sim_itree_indC_spec. econs 4; eauto. gbase. eauto. }
+    { guclo sim_itree_indC_spec. econs 5; eauto. gbase. eauto. }
+    { guclo sim_itree_indC_spec. econs 6; eauto. des. esplits; eauto. gbase. eauto. }
+    { guclo sim_itree_indC_spec. econs 7; eauto. gbase. eauto. }
+    { guclo sim_itree_indC_spec. econs 8; eauto. gbase. eauto. }
+    { guclo sim_itree_indC_spec. econs 9; eauto. des. esplits; eauto. gbase. eauto. }
+    { guclo sim_itree_indC_spec. econs 10; eauto. gbase. eauto. }
+    { guclo sim_itree_indC_spec. econs 11; eauto.  gbase. eauto. }
+  Qed.
+
+  Lemma sim_itreeC_spec r g
+    :
+      @sim_itreeC (gpaco8 (_sim_itree) (cpn8 _sim_itree) r g) (gpaco8 (_sim_itree) (cpn8 _sim_itree) g g)
+      <8=
+      gpaco8 (_sim_itree) (cpn8 _sim_itree) r g.
+  Proof.
+    i. eapply gpaco8_gpaco; [eauto with paco|].
+    eapply gpaco8_mon.
+    { eapply sim_itreeC_spec_aux. eauto. }
+    { auto. }
+    { i. eapply gupaco8_mon; eauto. }
+  Qed.
+
+  Lemma sim_itree_progress_flag R0 R1 RR w r g st_src0 st_tgt0
+        (SIM: gpaco8 _sim_itree (cpn8 _sim_itree) g g R0 R1 RR false false w st_src0 st_tgt0)
+    :
+      gpaco8 _sim_itree (cpn8 _sim_itree) r g R0 R1 RR true true w st_src0 st_tgt0.
+  Proof.
+    gstep. destruct st_src0, st_tgt0. econs; eauto. 
+  Qed.
+
+  Lemma sim_itree_flag_mon
+        (sim_itree: forall (R_src R_tgt: Type)
+                           (RR: st_local -> st_local -> R_src -> R_tgt -> Prop), bool -> bool -> world -> st_local * itree Es R_src -> st_local * itree Es R_tgt -> Prop)
+        R_src R_tgt (RR: st_local -> st_local -> R_src -> R_tgt -> Prop)
+        f_src0 f_tgt0 f_src1 f_tgt1 w st_src0 st_tgt0
+        (SIM: @_sim_itree sim_itree _ _ RR f_src0 f_tgt0 w st_src0 st_tgt0)
+        (SRC: f_src0 = true -> f_src1 = true)
+        (TGT: f_tgt0 = true -> f_tgt1 = true)
+    :
+      @_sim_itree sim_itree _ _ RR f_src1 f_tgt1 w st_src0 st_tgt0.
+  Proof.
+    revert f_src1 f_tgt1 SRC TGT.
+    induction SIM using _sim_itree_ind2; i; clarify.
+    { econs 1; eauto. }
+    { econs 2; eauto. }
+    { econs 3; eauto. }
+    { econs 4; eauto. }
+    { econs 5; eauto. } 
+    { econs 6; eauto. des. esplits; eauto. }
+    { econs 7; eauto. i. exploit K; eauto. i. des. eauto. }
+    { econs 8; eauto. i. exploit K; eauto. i. des. eauto. }
+    { econs 9; eauto. des. esplits; eauto. }
+    { econs 10; eauto. }
+    { econs 11; eauto. } 
+    { exploit SRC0; auto. exploit TGT0; auto. i. clarify. econs; eauto. }
+  Qed.
+
+
+  Definition sim_fsem: relation ( Any.t -> itree Es Any.t) :=
+    (eq ==> (fun it_src it_tgt => forall w mrs_src mrs_tgt (SIMMRS: wf w (mrs_src, mrs_tgt)),
+                 sim_itree false false w (mrs_src, it_src)
+                           (mrs_tgt, it_tgt)))%signature
+  .
+
+  Definition sim_fnsem: relation (gname -> option (Any.t -> itree Es Any.t)) := 
+   fun f g => forall s, match (f s), (g s) with
+                        | Some x, Some y => sim_fsem x y
+                        | None, None => True
+                        | _, _ => False
+                        end
+    .
+
+  Variant lflagC (r: forall (R_src R_tgt: Type)
+    (RR: st_local -> st_local -> R_src -> R_tgt -> Prop), bool -> bool -> world -> st_local * itree Es R_src -> st_local * itree Es R_tgt -> Prop)
+          {R_src R_tgt} (RR: st_local -> st_local -> R_src -> R_tgt -> Prop)
+    : bool -> bool -> world -> st_local * itree Es R_src -> st_local * itree Es R_tgt -> Prop :=
+  | lflagC_intro
+      f_src0 f_src1 f_tgt0 f_tgt1 w st_src st_tgt
+      (SIM: r _ _ RR f_src0 f_tgt0 w st_src st_tgt)
+      (SRC: f_src0 = true -> f_src1 = true)
+      (TGT: f_tgt0 = true -> f_tgt1 = true)
+    :
+      lflagC r RR f_src1 f_tgt1 w st_src st_tgt
+  .
+
+  Lemma lflagC_mon
+        r1 r2
+        (LE: r1  <8= r2)
+    :
+      @lflagC r1  <8= @lflagC r2
+  .
+  Proof. ii. destruct PR; econs; et. Qed.
+
+  Hint Resolve lflagC_mon: paco.
+
+  Lemma lflagC_spec: lflagC  <9= gupaco8 (_sim_itree) (cpn8 _sim_itree).
+  Proof.
+    eapply wrespect8_uclo; eauto with paco.
+    econs; eauto with paco. i. inv PR.
+    eapply GF in SIM.
+    revert x3 x4 SRC TGT. induction SIM using _sim_itree_ind2; i; clarify.
+    { econs 1; eauto. }
+    { econs 2; eauto. i. exploit K; eauto. i. des.
+      esplits; eauto. eapply rclo8_base. eauto. }
+    { econs 3; eauto. i. eapply rclo8_base. eauto. }
+    { econs 4; eauto. }
+    { econs 5; eauto. }
+    { econs 6; eauto.  des. esplits; eauto. }
+    { econs 7; eauto. i. exploit K; eauto. i. des. esplits; eauto. }
+    { econs 8; eauto. i. exploit K; eauto. i. des. esplits; eauto. }
+    { econs 9; eauto. des. esplits; eauto. }
+    { econs 10; eauto. }
+    { econs 11; eauto. }
+    { exploit SRC0; auto. exploit TGT0; auto. i. clarify. econs 12; eauto.
+      eapply rclo8_base; auto. }
+  Qed.
+
+  Lemma sim_itree_flag_down  R0 R1 RR r g w st_src0 st_tgt0 f_src f_tgt
+        (SIM: gpaco8 _sim_itree (cpn8 _sim_itree) r g R0 R1 RR false false w st_src0 st_tgt0)
+    :
+      gpaco8 _sim_itree (cpn8 _sim_itree) r g R0 R1 RR f_src f_tgt w st_src0 st_tgt0.
+  Proof.
+    guclo lflagC_spec. econs; eauto.
+  Qed.
+
+  Lemma sim_itree_bot_flag_up  R0 R1 RR w st_src0 st_tgt0 f_src f_tgt
+        (SIM: paco8 _sim_itree bot8 R0 R1 RR true true w st_src0 st_tgt0)
+    :
+      paco8 _sim_itree bot8 R0 R1 RR f_src f_tgt w st_src0 st_tgt0.
+  Proof.
+    ginit. remember true in SIM at 1. remember true in SIM at 1.
+    clear Heqb Heqb0. revert w st_src0 st_tgt0 f_src f_tgt b b0 SIM.
+    gcofix CIH. 
+    i. revert f_src f_tgt.
+
+    (* TODO: why induction using sim_itree_ind doesn't work? *)
+    pattern b, b0, w, st_src0, st_tgt0.
+    match goal with
+    | |- ?P b b0 w st_src0 st_tgt0 => set P
+    end.
+    revert b b0 w st_src0 st_tgt0 SIM.
+    eapply (@sim_itree_ind R0 R1 RR P); subst P; ss; i; clarify.
+    { guclo sim_itree_indC_spec. econs 1; eauto. }
+    { gstep. econs 2; eauto. i. gbase. eapply CIH; eauto. }
+    { gstep. econs 3; eauto. i. gbase. eapply CIH; eauto. }
+    { guclo sim_itree_indC_spec. econs 4; eauto. }
+    { guclo sim_itree_indC_spec. econs 5; eauto. } 
+    { guclo sim_itree_indC_spec. econs 6; eauto. des. esplits; eauto. }
+    { guclo sim_itree_indC_spec. econs 7; eauto. i. hexploit K; eauto. i. des. esplits; eauto. }
+    { guclo sim_itree_indC_spec. econs 8; eauto. i. hexploit K; eauto. i. des. esplits; eauto. }
+    { guclo sim_itree_indC_spec. econs 9; eauto. des. esplits; eauto. }
+    { guclo sim_itree_indC_spec. econs 10; eauto. } 
+    { guclo sim_itree_indC_spec. econs 11; eauto. } 
+    { eapply sim_itree_flag_down. gfinal. right.
+      eapply paco8_mon; eauto. ss.
+    }
+  Qed.
+
+  Variant lbindR (r s: forall S_src S_tgt (SS: st_local -> st_local -> S_src -> S_tgt -> Prop), bool -> bool -> world -> st_local * itree Es S_src -> st_local * itree Es S_tgt -> Prop):
+    forall S_src S_tgt (SS: st_local -> st_local -> S_src -> S_tgt -> Prop), bool -> bool -> world -> st_local * itree Es S_src -> st_local * itree Es S_tgt -> Prop :=
+  | lbindR_intro
+      f_src f_tgt w0 w1
+      R_src R_tgt RR
+      (st_src0 st_tgt0: st_local)
+      (i_src: itree Es R_src) (i_tgt: itree Es R_tgt)
+      (SIM: r _ _ RR f_src f_tgt w0 (st_src0, i_src) (st_tgt0, i_tgt))
+
+      S_src S_tgt SS
+      (k_src: ktree Es R_src S_src) (k_tgt: ktree Es R_tgt S_tgt)
+      (SIMK: forall st_src1 st_tgt1 vret_src vret_tgt (SIM: RR st_src1 st_tgt1 vret_src vret_tgt), s _ _ SS false false w1 (st_src1, k_src vret_src) (st_tgt1, k_tgt vret_tgt))
+    :
+      lbindR r s SS f_src f_tgt w1 (st_src0, ITree.bind i_src k_src) (st_tgt0, ITree.bind i_tgt k_tgt)
+  .
+
+  Hint Constructors lbindR: core.
+
+  Lemma lbindR_mon 
+        r1 r2 s1 s2
+        (LEr: r1  <8= r2) (LEs: s1  <8= s2)
+    :
+      lbindR r1 s1  <8= lbindR r2 s2
+  .
+  Proof. ii. destruct PR; econs; et. Qed.
+
+  Definition lbindC r := lbindR r r.
+  Hint Unfold lbindC: core.
+
+  Lemma lbindC_wrespectful: wrespectful8 (_sim_itree) lbindC.
+  Proof.
+    econs.
+    { ii. eapply lbindR_mon; eauto. }
+    i. rename l into llll. inv PR; csc.
+    remember (st_src0, i_src). remember(st_tgt0, i_tgt).
+    revert st_src0 i_src st_tgt0 i_tgt Heqp Heqp0.
+    revert k_src k_tgt SIMK. eapply GF in SIM.
+    induction SIM using _sim_itree_ind2; i; clarify.
+    + rewrite ! bind_ret_l. exploit SIMK; eauto. i.
+      eapply sim_itree_flag_mon.
+      { eapply sim_itree_mon; eauto. i. eapply rclo8_base. auto. }
+      { ss. }
+      { ss. }
+    + rewrite ! bind_bind. econs; eauto. i.
+      eapply rclo8_clo_base. econs; eauto.
+    + rewrite ! bind_bind. econs; eauto. i.
+      eapply rclo8_clo_base. econs; eauto.
+    + rewrite ! bind_tau. econs; eauto.
+    + rewrite ! bind_tau. econs; eauto.
+    + rewrite ! bind_bind. econs; eauto. des. esplits; eauto.
+    + rewrite ! bind_bind. econs; eauto. i. exploit K; eauto. i. des. esplits; eauto.
+    + rewrite ! bind_bind. econs; eauto. i. exploit K; eauto. i. des. esplits; eauto.
+    + rewrite ! bind_bind. econs; eauto. des. esplits; eauto.
+    + rewrite ! bind_bind. econs; eauto. 
+    + rewrite ! bind_bind. econs; eauto. 
+    + econs; eauto. eapply rclo8_clo_base. econs; eauto.
+  Qed.
+
+  Lemma lbindC_spec: lbindC  <9= gupaco8 (_sim_itree) (cpn8 (_sim_itree)).
+  Proof.
+    intros. eapply wrespect8_uclo; eauto with paco. eapply lbindC_wrespectful.
+  Qed.
+
+End SIM.
+
+Require Import SimGlobal.
+Require Import Red IRed.
+
+Module TAC.
+  Ltac ired_l := try (prw _red_gen 2 0).
+  Ltac ired_r := try (prw _red_gen 1 0).
+
+  Ltac ired_both := ired_l; ired_r.
+
+  Ltac step := ired_both; guclo simg_safe_spec; econs; et; i.
+  Ltac steps := (repeat step); ired_both.
+
+  Ltac force := ired_both; guclo simg_indC_spec; econs; et.
+End TAC.
+Import TAC.
+
+
+Section PRODUCT_LENS.
+
+  (* Context {A B : Type}. *)
+
+  Definition fstl : Lens.t Any.t Any.t :=
+    (fun ab => 
+      match Any.split ab with
+      | Some (a, b) => (a, (fun a' => Any.pair a' b)) 
+      | None => (tt↑, (fun _ => ab))
+      end).
+
+  Definition sndl : Lens.t Any.t Any.t :=
+    (fun ab => 
+      match Any.split ab with
+      | Some (a, b) => (b, (fun b' => Any.pair a b')) 
+      | None => (tt↑, (fun _ => ab))
+      end).
+
+End PRODUCT_LENS.
 
 Module ModSemAdd.
 Import ModSem.
@@ -17,12 +839,44 @@ Import ModSem.
 Section ADD.
   Variable M1 M2 : t.
 
+  Definition run_l {V} (run: Any.t -> Any.t * V): Any.t -> Any.t * V :=
+    fun st => 
+      match Any.split st with
+      | Some (a, b) => let (a', v) := run a in (Any.pair a' b, v)
+      | None => run tt↑
+        (* (tt↑, snd (run tt↑)) *)
+      end.
+ 
+  Definition run_r {V} (run: Any.t -> Any.t * V): Any.t -> Any.t * V :=
+    fun st => 
+      match Any.split st with
+      | Some (a, b) => let (b', v) := run b in (Any.pair a b', v)
+      | None => run tt↑
+      (* (tt↑, snd (run tt↑)) *)
+      end.      
+
   Definition emb_l : forall T, Es T -> Es T :=
-    lmap fstl.
+    fun T es => 
+    match es with
+    | inr1 (inl1 (SUpdate run)) => inr1 (inl1 (SUpdate (run_l run)))
+    | _ => es
+    end.   
 
   Definition emb_r : forall T, Es T -> Es T :=
-    lmap sndl.
+    fun T es => 
+    match es with
+    | inr1 (inl1 (SUpdate run)) => inr1 (inl1 (SUpdate (run_r run)))
+    | _ => es
+    end. 
 
+  Definition trans_l f : gname * (Any.t -> itree _ Any.t) :=
+    (fst f, (fun args => translate emb_l ((snd f) args))).
+
+  Definition trans_r f : gname * (Any.t -> itree _ Any.t) :=
+    (fst f, (fun args => translate emb_r ((snd f) args))).   
+
+  (* Definition add_fnsems : alist gname (Any.t -> itree _ Any.t) :=
+    (List.map trans_l M1.(fnsems)) ++ (List.map trans_r M2.(fnsems)). *)
 
   Definition add_fnsems : gname -> option (Any.t -> itree _ Any.t) :=
     fun fn =>
@@ -44,13 +898,13 @@ End ADD.
 
 Section PROOF.
 
-Definition swap ab: Any.t :=
+Definition swap (ab: Any.t) : Any.t :=
   match Any.split ab with
   | Some (a, b) => Any.pair b a
   | None => ab (* or UB? *)
   end.
 
-Definition swap_state {X} (f: Any.t -> Any.t * X)  :=
+Definition swap_state {X} (f: Any.t -> Any.t * X): Any.t -> Any.t * X  :=
   (fun ba => let '(ab', t) := f (swap ba) in ((swap ab'), t)).
 
 Definition swap_Es T (es: Es T) : Es T :=
@@ -78,81 +932,251 @@ Definition swap_ems {R} (itl: itree Es R) (itr: itree Es R) :=
   end. *)
 
 
-(* 
-Definition assoc a'bc: Any.t :=
+
+
+(* Definition assoc' (a'bc: Any.t): Any.t :=
   match Any.split a'bc with
   | Some (a, bc) => 
       match Any.split bc with
-      | Some (b, c) => (Any.pair (Any.pair a b) c)
-      | None => (a'bc) (* or UB? *)
+      | Some (b, c) => Any.pair (Any.pair a b) c
+      | None => a'bc
       end
-    |None => (a'bc) (* or UB? *)
+    |None => a'bc
   end
-  . 
+  . *)
   
-Definition assoc' ab'c: Any.t :=
-  match Any.split ab'c with
+  Definition assoc (abc: Any.t) (abc': Any.t): Prop :=
+  match Any.split abc with
   | Some (ab, c) => 
       match Any.split ab with
-      | Some (a, b) => (Any.pair a (Any.pair b c))
-      | None => (ab'c) (* or UB? *)
+      | Some (a, b) => abc' = Any.pair a (Any.pair b c)
+      | None => False
       end
-    |None => (ab'c) (* or UB? *)
+    |None => False
   end
   . 
 
-Definition assoc_state {X} (f: Any.t -> Any.t * X) :=
-  (fun ab'c => let '(a'bc, t) := f (assoc' ab'c) in (assoc a'bc, t)).
+  (* Lemma assoc_any (a b c: Any.t) :
+    assoc (Any.pair (Any.pair a b) c) (Any.pair a (Any.pair b c))
+  .
+  Proof.
+    unfold assoc. rewrite ! Any.pair_split. refl.
+  Qed.
 
-Definition assoc_Es T (es: Es T) : Es T :=
+  (* Definition assoc (abc: Any.t) (abc': Any.t): Prop :=
+  match Any.split abc with
+  | Some (a, bc) => 
+      match Any.split bc with
+      | Some (b, c) => abc' = Any.pair (Any.pair a b) c
+      | None => True
+      end
+    |None => True
+  end
+  . 
+  *)
+
+  Lemma assoc_any (a b c: Any.t) :
+    assoc (Any.pair a (Any.pair b c)) (Any.pair (Any.pair a b) c)
+  .
+  Proof.
+    unfold assoc. rewrite ! Any.pair_split. refl.
+  Qed. *)
+
+
+  Definition is_pair: Any.t -> Any.t :=
+    fun x => match Any.split x with
+            | Some (_, _) => x
+            | None => tt↑
+            end.
+
+(* Definition assoc_state_0 T (f: Any.t -> Any.t * T): Any.t -> Any.t * T :=
+  (fun ab'c => 
+    match Any.split ab'c with
+    | Some (ab, c) => 
+        match Any.split ab with
+        | Some (a, b) => 
+            let '(a'bc, t) := f (Any.pair a (Any.pair b c)) in
+            (assoc' a'bc, t)
+        | None => 
+            (* (ab'c, snd (f ab)) *)
+            (Any.pair tt↑ c, snd (f tt↑))
+        end
+    | None => f tt↑
+      (* (ab'c, snd (f ab'c)) *)
+    end). *)
+
+Definition assoc_any_l (abc: Any.t): option Any.t :=
+  match Any.split abc with
+  | None => None
+  | Some (a, bc) => 
+      match Any.split bc with
+      | None => None
+      | Some (b, c) => Some (Any.pair (Any.pair a b) c)
+      end
+  end.
+
+  Definition assoc_any_r (abc: Any.t): option Any.t :=
+    match Any.split abc with
+    | None => None
+    | Some (ab, c) => 
+        match Any.split ab with
+        | None => None
+        | Some (a, b) => Some (Any.pair a (Any.pair b c))
+        end
+    end.
+    
+Definition assoc_state V (f: Any.t -> Any.t * V): Any.t -> Any.t * V :=
+  fun abc =>
+    match assoc_any_r abc with
+    | None => f tt↑
+        (* (tt↑, snd (f tt↑)) *)
+    | Some abc' => 
+        let '(r, v) := f abc' in 
+        match assoc_any_l r with
+        | None => f tt↑
+          (* (tt↑, v) *)
+        | Some r' => (r', v)
+        end
+    end.
+
+
+(* Definition assoc_state T (f: Any.t -> Any.t * T): Any.t -> Any.t * T :=
+  fun abc =>
+    match Any.split abc with
+    | None => (tt↑, snd (f tt↑))
+    | Some (ab, c) =>
+        match Any.split ab with
+        | None => (tt↑, snd (f tt↑))
+        | Some (a, b) => 
+          let '(a'bc, t) := f (Any.pair a (Any.pair b c)) in
+        (assoc' a'bc, t)
+
+
+Definition assoc_state T (f: Any.t -> Any.t * T): Any.t -> Any.t * T :=
+  (fun ab'c => 
+    match Any.split ab'c with
+    | Some (ab, c) => 
+        match Any.split ab with
+        | Some (a, b) => 
+            let '(a'bc, t) := f (Any.pair a (Any.pair b c)) in
+            (assoc' a'bc, t)
+        | None => 
+            let '(c', t) := f (Any.pair tt↑ (Any.pair tt↑ c)) in
+            let c' := assoc' c' in
+            let c' := match Any.split c' with
+                    | Some (_, c') => c'
+                    | None => c'
+                    end in
+            (Any.pair ab c', t)
+            (* (Any.pair ab (fst (f c)), snd (f c)) *)
+            (* (Any.pair tt↑ c, snd (f tt↑)) *)
+        end
+    | None => 
+      let '(c', t) := f ab'c in
+      (* let c' := assoc' c' in *)
+      let c := match Any.split c' with
+              | Some (_, c') => c'
+              | None => c'
+              end in
+      (c', snd (f ab'c))
+    end).     *)
+(* Definition assoc_state {X} (f: Any.t -> Any.t * X): Any.t -> Any.t * X :=
+  (fun ab'c => let '(a'bc, t) := f (assoc' ab'c) in (assoc a'bc, t)). *)
+
+(* Definition assoc_run {T} (f f': Any.t -> Any.t * T) : Prop :=
+  (exists a b c,
+    let abc := Any.pair a (Any.pair b c) in
+    let abc' := Any.pair (Any.pair a b) c in 
+    assoc (fst (f abc)) (fst (f' abc')) /\ 
+                snd (f abc) = snd (f' abc'))
+    (* (exists abc abc', assoc abc abc' /\ assoc (fst (f abc)) (fst (f' abc')) /\ snd (f abc) = snd (f' abc')) *)
+
+. *)
+
+(* Definition assoc_Es T (es: Es T) (es': Es T) : Prop :=
+  match es, es' with
+  | (inr1 (inl1 (SUpdate f))), (inr1 (inl1 (SUpdate f')))  => assoc_run f f'
+  | (inr1 (inr1 x)), (inr1 (inr1 x')) => True
+  | (inl1 y), (inl1 y') => True
+  | _, _ => False
+  end. *)
+
+
+(* Definition assoc_Es' assoc_state T (es: Es T) : Es T :=
   match es with
-  | inr1 (inl1 (SUpdate f)) => inr1 (inl1 (SUpdate (assoc_state f)))
+  | inr1 (inl1 (SUpdate f)) => inr1 (inl1 (SUpdate (assoc_state _ f)))
   | inr1 (inr1 x) => inr1 (inr1 x)
   | inl1 y => inl1 y
-  end.
-  
-Definition assoc_ems {R} (itl: itree Es R) (itr: itree Es R) :=
-  itr = translate assoc_Es itl.  *)
+  end.   *)
+
+  Definition assoc_Es T (es: Es T) : Es T :=
+    match es with
+    | inr1 (inl1 (SUpdate f)) => inr1 (inl1 (SUpdate (assoc_state f)))
+    | _ => es
+    end.
+
+Variable it: itree Es Any.t.
+Check translate (emb_l >>> emb_l) it.
+Check emb_l = (emb_l >>> emb_l).
+
+Inductive assoc_emb : IFun Es Es -> IFun Es Es -> Prop := 
+  |assoc_emb_1 : assoc_emb emb_l (emb_l >>> emb_l)
+  |assoc_emb_2 : assoc_emb (emb_l >>> emb_r ) (emb_r >>> emb_l)
+  |assoc_emb_3 : assoc_emb (emb_r >>> emb_r) emb_r
+.
+
+Inductive assoc_ems : itree Es Any.t -> itree Es Any.t -> Prop := 
+  | assoc_ems_intro emb_l emb_r it (EMB: assoc_emb emb_l emb_r) :
+      assoc_ems (translate emb_l it) (translate emb_r it).
 
 
+
+
+(* Definition assoc_ems {R} (itl: itree Es R) (itr: itree Es R) :=
+  translate (assoc_Es) itl = itr. *)
+
+
+  (* (exists f, itr = translate (assoc_Es' f) itl) . *)
+  (* /\ (forall T, exists f, forall es, assoc_Es es ((assoc_Es' f) T es)).  *)
+
+(* Print trigger. *)
+
+(* Search translate. *)
 
 Lemma translate_triggerUB T (f: forall T, Es T -> Es T) (g: forall T, (Any.t -> Any.t * T) -> (Any.t -> Any.t * T))
-      (F: f = (fun _ es => match es with
-                        | inr1 (inl1 (SUpdate run)) => inr1 (inl1 (SUpdate (g _ run)))
-                        | inr1 (inr1 x) => inr1 (inr1 x)
-                        | inl1 y => inl1 y
-                 end))
+    (COND: f _ (subevent _ (Take void)) = (subevent _ (Take void)))
   :
-      @triggerUB _ T _ = translate f (@triggerUB _ T _)
+      translate f (@triggerUB _ T _) = @triggerUB _ T _ 
 .
+
 Proof.
   unfold triggerUB.
   erewrite ! (bisimulation_is_eq _ _ (translate_bind _ _ _)).
   f_equal.
-  - unfold trigger. rewrite F.
+  - unfold trigger. 
     erewrite ! (bisimulation_is_eq _ _ (translate_vis _ _ _ _)).
-    repeat f_equal.
+    repeat f_equal; et. 
     extensionality v. destruct v.
   - extensionality v. destruct v.
 Qed. 
 
 
-Lemma swap_swap a : swap (swap a) = a.
+(* Lemma swap_swap a : swap (swap a) = a.
 Proof.
   i. unfold swap.
   destruct (Any.split a) eqn:A.
   - destruct p. rewrite Any.pair_split. 
     rewrite <- Any.split_pair with (a:=a); et.
   - rewrite A. et.  
-Qed.
+Qed. *)
 
 
 Lemma swap_ems_prog X ms0 ms1 (e: callE X)
 :
       swap_ems (prog (add ms1 ms0) e) (prog (add ms0 ms1) e)
 .
-Proof. 
-  destruct e. s. unfold unwrapU, add_fnsems. 
+Proof. Admitted.
+  (* destruct e. s. unfold unwrapU, add_fnsems. 
   des_ifs; grind; unfold swap_ems.
   - eapply translate_triggerUB; ss.
   - erewrite <- ! (bisimulation_is_eq _ _ (translate_cmpE _ _ _ _ _ _ _)).
@@ -203,134 +1227,137 @@ Proof.
       repeat f_equal.
       extensionality v. destruct v.
     + extensionality v. destruct v.
-Qed.
+Qed. *)
 
 
-(* Lemma assoc_ems_prog X ms0 ms1 ms2 (e: callE X)
+
+Lemma assoc_ems_prog ms0 ms1 ms2 (e: callE Any.t)
 
 :
   assoc_ems (prog (add ms0 (add ms1 ms2)) e) (prog (add (add ms0 ms1) ms2) e)
 .
-Proof.
-  destruct e. s. 
+Proof. Admitted.
+  (* destruct e. s. 
   unfold unwrapU.
+  unfold assoc_ems. 
   repeat (unfold add_fnsems; grind).
-  des_ifs; grind; unfold assoc_ems.
-  - eapply translate_triggerUB. ss. 
-  - eapply translate_triggerUB. ss.
+  (* splits. *)
+  (* 2: {
+    exists (init_st (add ms0 (add ms1 ms2))).
+    exists (init_st (add (add ms0 ms1) ms2)).
+    split.
+    - apply assoc_any.
+    - s. unfold assoc_Es' in *. inv Heq.
+      unfold assoc_state. rewrite ! Any.pair_split. des_ifs.
+      unfold assoc, assoc'. des_ifs; et; inv Heq1; clarify.
+      + split; et. admit.
+      + split; et. admit.
+  }  *)
+  des_ifs; grind; try (repeat (rewrite translate_triggerUB; et)). (* exists assoc_state_1 removed*)
+
   - erewrite <- ! (bisimulation_is_eq _ _ (translate_cmpE _ _ _ _ _ _ _)).
+    f_equal.
+    unfold ">>>", Cat_IFun.
+    (* unfold emb_l. *)
+    extensionalities T es.
+    unfold emb_l.
+    des_ifs. s.
+    
+    repeat f_equal. i.
+    unfold run_l, assoc_state.
+    extensionality abc.
+    (* unfold assoc_state. s.
+    extensionality ab'c.
+    unfold lens_state. s.
+    unfold Lens.set, Lens.view.
+    unfold fstl. *)
+    destruct (Any.split abc) eqn: ABC; cycle 1.
+    + rewrite ! Any.upcast_split.
+      unfold assoc_any_r. rewrite ABC. et.
+    + destruct p as [ab c]. s.
+      unfold assoc_any_r. rewrite ABC.
+      (* unfold assoc'. *)
+      destruct (Any.split ab) eqn:AB; cycle 1.
+      * rewrite ! Any.upcast_split. s.
+         unfold assoc_any_l, assoc_any_r.
+        rewrite ABC. ss.
+      * destruct p as [a b]. s. rewrite Any.pair_split.
+        des_ifs; ss; rewrite ! Any.pair_split in *; clarify; rewrite ! Any.pair_split in *; clarify.
+      * s. rewrite Any.pair_split. s. rewrite ! Any.pair_split. et. 
+        (* admit.  *)
+        (* rewrite Any.upcast_split. s. et.  *)
+        (* rewrite Any.pair_split. ss. *)
+    + s. 
+      (* admit. *)
+      (* s. rewrite AB'C. et. *)
+      s. rewrite Any.upcast_split. et. 
+           
+
+  - 
+    erewrite <- ! (bisimulation_is_eq _ _ (translate_cmpE _ _ _ _ _ _ _)).
     eapply translate_triggerUB.
     unfold ">>>".
     unfold Cat_IFun.
     extensionalities T es. des_ifs.
-    (* destruct es as [c|[s|e]]; unfold emb_r, lmap; et.
-    destruct s. s.
-    repeat f_equal.
-    unfold assoc_state. s. 
-    (* destruct SUpdate.  *)
-    extensionality x. destruct x, p. 
-    instantiate (1 := (fun _ run '(s0, s1, s2) => (s0, fst (fst (run (s1, s2) )), snd (fst (run (s1, s2))), snd (run (s1, s2))))).
-     s. unfold Lens.view. des_ifs. ss.
-    rewrite Heq. et. *)
-  - erewrite <- translate_triggerUB with (f:=assoc_Es); ss.
-    symmetry.
-    eapply translate_triggerUB.
-    unfold emb_l, lmap.
-    extensionalities T es. des_ifs.
-  - erewrite <- ! (bisimulation_is_eq _ _ (translate_cmpE _ _ _ _ _ _ _)).
 
-    f_equal.
-    unfold ">>>", Cat_IFun.
-    unfold emb_l, lmap.
-    extensionalities T es. des_ifs. s.
-    destruct s1. s.
-
-    repeat f_equal. 
-    unfold assoc_state. s.
-    extensionality ab'c.
-    unfold lens_state. s.
-    unfold Lens.set, Lens.view.
-    (* unfold fstl, sndl. *)
-    (* unfold assoc, assoc'. *)
-    f_equal.
-    + unfold fstl. 
-      destruct (Any.split ab'c) eqn:AB'C. 
-      * destruct p as [ab c]. s.
-        unfold assoc. 
-        destruct (Any.split ab) eqn:AB.
-        -- destruct p as [a b]. s.
-           unfold assoc'. des_ifs; ss; clarify.
-           4: { rewrite Any.upcast_split in Heq. inv Heq. }
-           5: { admit. }
-           all: admit.
-        -- s. unfold assoc'. des_ifs; ss; clarify.
-          ++ rewrite Any.pair_split in Heq.
-        destruct (Any.split (assoc' ab'c)) eqn:A'BC. 
-        -- destruct p.
-          (* At this point, split t0, split t3 shouldn't be None. *)
-           s. rewrite Any.pair_split.
-           unfold assoc' in *. rewrite AB'C in A'BC.
-           destruct (Any.split t0) eqn:T0. destruct p.
-           rewrite Any.pair_split in A'BC. inv A'BC.
-           ++ s. rewrite Any.pair_split. et. 
-           ++ s. destruct (Any.split t3) eqn:T3. destruct p.
-            ** destruct p
-            --- destruct p. s. rewrite Any.pair_split in X'.
-                inv X'. rewrite Any.pair_split in T3. inv T3. et.
-            --- s. rewrite X' in X. inv X.
-
-    s. destruct (Any.split x) eqn:X.
-    + destruct p. s.
-      destruct (Any.split t0) eqn:T0.
-      * destruct p. s.
-      unfold assoc_state, assoc. des_ifs.
-        f_equal.
-        -- s. f_equal.
-           ++ f_equal.
-      
-      destruct (Any.split t2) eqn:T2.
-        -- destruct p. s. rewrite Any.pair_split. s.
-           destruct (Any.split t1) eqn:T1.
-           ++ destruct p. s.
-           f_equal.
-           ++ 
-     
-    
-    destruct (run (fst (fstl (fst (fstl (Some t0)))))) eqn: T0.
-      (* destruct (run (fst (fstl (assoc (Some t0))))) eqn: Assoc0. *)
-      s. destruct (Any.split t0) eqn:T1.
-      * destruct p. s.
-        destruct (Any.split t2) eqn:T2.
-        -- destruct (Any.split t3) eqn: T3.
-          ++ destruct p, p0. s. rewrite Any.pair_split. s.   
-             f_equal.
-      f_equal.
-      * s. destruct (Any.split t0) eqn:T1.
-        -- destruct p. f_equal. s. 
-      * destruct p. s. destruct (Any.split t1) eqn: T1.
-        -- destruct p. ss. destruct (Any.split t2) eqn: T2.
-          ++ destruct p. ss. rewrite ! Any.pair_split. ss.
-    unfold lens_state. s. 
-    f_equal.
-    (* Set Printing All.  *)
-  - erewrite <- ! (bisimulation_is_eq _ _ (translate_cmpE _ _ _ _ _ _ _)).
+  - 
+    erewrite <- ! (bisimulation_is_eq _ _ (translate_cmpE _ _ _ _ _ _ _)).
     f_equal.
     unfold ">>>", Cat_IFun, emb_l, emb_r, lmap.
     extensionalities T es. des_ifs.
     destruct s2. s.
     repeat f_equal.
-    extensionality x. destruct x, p. 
-    s. des_ifs.
-  - erewrite <- ! (bisimulation_is_eq _ _ (translate_cmpE _ _ _ _ _ _ _)).
+    unfold assoc_state. s.
+    extensionality ab'c.
+    unfold lens_state. s.
+    unfold Lens.set, Lens.view.
+    unfold fstl, sndl.
+    destruct (Any.split ab'c) eqn: AB'C.
+    + destruct p as [ab c]. s.
+      unfold assoc'.
+      destruct (Any.split ab) eqn:AB.
+      * destruct p as [a b]. s. rewrite Any.pair_split.
+        des_ifs; ss; rewrite ! Any.pair_split in *; clarify; rewrite ! Any.pair_split in *; clarify.
+      * s.  
+        rewrite ! Any.pair_split. s. rewrite ! Any.pair_split. s.
+        rewrite ! Any.pair_split. refl. 
+        (* admit. *)
+        (* rewrite Any.upcast_split. s. rewrite Any.upcast_split. et. *)
+        (* rewrite ! Any.pair_split. ss. repeat f_equal. *)
+    + 
+      (* admit. *)
+      (* s. rewrite AB'C. et.  *)
+      s. rewrite Any.upcast_split. refl.
+      (* s. rewrite Any.upcast_split. et.  *)
+
+  - 
+    erewrite <- ! (bisimulation_is_eq _ _ (translate_cmpE _ _ _ _ _ _ _)).
     f_equal.
     unfold ">>>", Cat_IFun, emb_r, lmap.
     extensionalities T es. des_ifs. 
     destruct s0. s.
     repeat f_equal. 
     unfold assoc_state, lens_state.
-    extensionality x. destruct x, p. s.
-    f_equal.
-  - unfold triggerUB. grind.
+    extensionality ab'c.
+    unfold Lens.set, Lens.view, fstl, sndl.
+    destruct (Any.split ab'c) eqn: AB'C.
+    + destruct p as [ab c].
+      unfold assoc'.
+      destruct (Any.split ab) eqn: AB.
+      * destruct p as [a b]. 
+        repeat (rewrite ! Any.pair_split; s).
+        repeat f_equal. apply Any.split_pair in AB. et.
+      * s. 
+        rewrite ! Any.pair_split. s. rewrite ! Any.pair_split. s.
+        rewrite ! Any.pair_split. et.
+        (* rewrite Any.upcast_split. s. rewrite Any.upcast_split. s. *)
+    + s. rewrite Any.upcast_split. s. et.
+      (* s. rewrite AB'C. et. *)
+      (* s. rewrite Any.upcast_split. s. rewrite Any.upcast_split. et. *)
+         
+
+  - 
+    unfold triggerUB. grind.
     erewrite ! (bisimulation_is_eq _ _ (translate_bind _ _ _)).
     f_equal.
     + unfold trigger.
@@ -339,6 +1366,113 @@ Proof.
       extensionality v. destruct v.
     + extensionality v. destruct v.
 Qed. *)
+
+Definition assoc_st (stp: Any.t * Any.t) : Prop :=
+  exists a b c, fst stp = Any.pair a (Any.pair b c) /\ 
+  snd stp = Any.pair (Any.pair a b) c
+.
+(* Check sim_itree. *)
+Hint Resolve sim_itree_mon: paco.
+Hint Resolve cpn8_wcompat: paco.
+
+
+
+Lemma add_assoc_aux
+        itl itr stl str
+        (ASSOC: assoc_ems itl itr)
+        (STATE: assoc_st (stl, str))
+
+  :
+      sim_itree (fun _ => assoc_st) top2 false false tt (stl, itl) (str, itr).
+Proof.
+  destruct ASSOC, STATE. des. ss.
+  (* unfold assoc_st. *)
+  ginit. 
+  generalize it0 as itr. 
+  clarify.
+  generalize x as a0.
+  generalize b as b0.
+  generalize c as c0.
+  gcofix CIH. i.
+  rewrite (itree_eta_ itr).
+  destruct (observe itr).
+  - erewrite ! (bisimulation_is_eq _ _ (translate_ret _ _)).
+    gstep. apply sim_itree_ret.
+    unfold lift_rel. 
+    exists tt. splits; et.
+    unfold assoc_st. exists a0, b0, c0; et.
+  - erewrite ! (bisimulation_is_eq _ _ (translate_tau _ _)).
+    gstep. 
+    apply sim_itree_tau_src. apply sim_itree_tau_tgt. 
+    eapply sim_itree_progress; et.
+    gfinal. left. eapply CIH; et.
+  - erewrite ! (bisimulation_is_eq _ _ (translate_vis _ _ _ _)).
+    rewrite <- ! bind_trigger.
+    destruct e as [c'|[s|e]].
+    + (* callE *)
+      gstep. destruct c', EMB. 
+      (* SIMPLIFY BELOW *)
+      * apply sim_itree_call; clarify.
+        -- exists a0, b0, c0; et.
+        -- i. destruct WF, H, H, H. ss. clarify.
+         gfinal. left. eapply CIH.
+      * apply sim_itree_call; clarify.
+        -- eexists a0, b0, c0; et.
+        -- i. unfold assoc_st in WF. des. ss. clarify.
+           gfinal. left. eapply CIH.
+      * apply sim_itree_call; clarify.
+        -- eexists a0, b0, c0; et.
+        -- i. unfold assoc_st in WF. des. ss. clarify.
+           gfinal. left. eapply CIH. 
+    + (* sE *)
+      gstep. destruct s, EMB.
+      * apply sim_itree_supdate_src. apply sim_itree_supdate_tgt.
+        eapply sim_itree_progress; et.
+        unfold run_l, run_r. rewrite ! Any.pair_split.
+        gfinal. left. destruct (run a0). eapply CIH.
+      * apply sim_itree_supdate_src. apply sim_itree_supdate_tgt.
+        eapply sim_itree_progress; et.
+        unfold run_l, run_r. rewrite ! Any.pair_split.
+        gfinal. left. destruct (run b0). eapply CIH.
+      * apply sim_itree_supdate_src. apply sim_itree_supdate_tgt.
+        eapply sim_itree_progress; et.
+        unfold run_l, run_r. rewrite ! Any.pair_split.
+        gfinal. left. destruct (run c0). eapply CIH.        
+    + (* eventE *)
+      gstep. destruct e, EMB.
+      (* Choose *)
+      * apply sim_itree_choose_tgt. i. apply sim_itree_choose_src. exists x0.
+        eapply sim_itree_progress; et.
+        gfinal. left. eapply CIH.
+      * apply sim_itree_choose_tgt. i. apply sim_itree_choose_src. exists x0.
+        eapply sim_itree_progress; et.
+        gfinal. left. eapply CIH.
+      * apply sim_itree_choose_tgt. i. apply sim_itree_choose_src. exists x0.
+        eapply sim_itree_progress; et.
+        gfinal. left. eapply CIH.
+      (* Take *)
+      * apply sim_itree_take_src. i. apply sim_itree_take_tgt. exists x0.
+        eapply sim_itree_progress; et.
+        gfinal. left. eapply CIH. 
+      * apply sim_itree_take_src. i. apply sim_itree_take_tgt. exists x0.
+        eapply sim_itree_progress; et.
+        gfinal. left. eapply CIH. 
+      * apply sim_itree_take_src. i. apply sim_itree_take_tgt. exists x0.
+        eapply sim_itree_progress; et.
+        gfinal. left. eapply CIH.
+      (* Syscall *)
+      * apply sim_itree_syscall. i.
+        eapply sim_itree_flag_down.
+        gfinal. left. eapply CIH. 
+      * apply sim_itree_syscall. i.
+        eapply sim_itree_flag_down.
+        gfinal. left. eapply CIH.
+      * apply sim_itree_syscall. i.
+        eapply sim_itree_flag_down.
+        gfinal. left. eapply CIH.
+Qed. 
+
+
 
 (* Move to SimGlobal? *)
 Lemma simg_map R0 R1 RR R0' R1' RR' f_src f_tgt itl itr (f0: R0 -> R0') (f1: R1 -> R1')
@@ -541,6 +1675,9 @@ Proof. Admitted.
 Qed. *) *)
 
 
+(* Variant _wf_run_itree (wf_run_itree: itree Es Any.t -> Prop) (itr: itree Es Any.t): Prop := *)
+  
+
 (* TODO: Define aux for both comm / assoc. *)
 Lemma add_assoc_aux
         ms0 ms1 ms2
@@ -549,17 +1686,32 @@ Lemma add_assoc_aux
         (snd <$> interp_Es (prog (add (add ms0 ms1) ms2)) (prog (add (add ms0 ms1) ms2) (Call "main" initial_arg)) (init_st (add (add ms0 ms1) ms2)))
         (snd <$> interp_Es (prog (add ms0 (add ms1 ms2))) (prog (add ms0 (add ms1 ms2)) (Call "main" initial_arg)) (init_st (add ms0 (add ms1 ms2))))
 .
-Proof. Admitted.
-  (* generalize (Call "main" initial_arg) as e.
-  assert (REL: assoc (init_st (add ms0 (add ms1 ms2))) = init_st (add (add ms0 ms1) ms2)).
-  { unfold init_st, assoc. ss. rewrite ! Any.pair_split. et. }
-  revert REL.
+Proof.
+ (* Admitted. *)
+  generalize (Call "main" initial_arg) as e.
+  (* assert (REL: assoc (init_st (add ms0 (add ms1 ms2))) (init_st (add (add ms0 ms1) ms2))).
+  { unfold init_st, assoc. ss. rewrite ! Any.pair_split. et. } *)
+  (* assert (REL: assoc' (init_st (add ms0 (add ms1 ms2))) = init_st (add (add ms0 ms1) ms2)). *)
+  (* { unfold init_st,  assoc. ss. rewrite ! Any.pair_split. refl. } *)
+  (* revert REL. *)
+  (* s. *)
+
+  (* assert (SPLIT: exists mst0 mst1 mst2,
+           Any.split (init_st (add ms0 (add ms1 ms2))) = Some (mst0, Any.pair mst1 mst2)).
+  { s. exists (init_st ms0), (init_st ms1), (init_st ms2).
+    splits; rewrite ! Any.pair_split; et. }
+  revert SPLIT. *)
+
+  (* s. *)
+  (* generalize (init_st ms0) as st0.
+  generalize (init_st ms1) as st1.
+  generalize (init_st ms2) as st2. *)
 
   generalize (init_st (add (add ms0 ms1) ms2)) as stl0.
   generalize (init_st (add ms0 (add ms1 ms2))) as str0.
 
   i. eapply simg_map.
-  2: { instantiate (1 := (fun r0 r1 => snd r0 = snd r1 /\ fst r0 = (assoc (fst r1)))).
+  2: { instantiate (1 := (fun r0 r1 => snd r0 = snd r1 /\ assoc (fst r0) (fst r1))).
        i. apply H. }
     
   revert_until ms2.
@@ -572,7 +1724,12 @@ Proof. Admitted.
   generalize (prog (add (add ms0 ms1) ms2) e) as itl.
   generalize (prog (add ms0 (add ms1 ms2)) e) as itr.
   rewrite <- REL.
+  revert SPLIT.
   generalize str0 as str.
+  generalize mst0 as mst0'.
+  generalize mst1 as mst1'.
+  generalize mst2 as mst2'.
+
 
   gcofix CIH'. i.
   inv REL'.
@@ -583,21 +1740,34 @@ Proof. Admitted.
   - (* Ret *)
     erewrite ! (bisimulation_is_eq _ _ (translate_ret _ _)).
     rewrite ! interp_Es_ret.
-    gstep. apply simg_ret. et.
+    gstep. apply simg_ret.
+    splits; et. s.
+    unfold assoc, assoc'. 
+    (* des_ifs. *)
+
+    rewrite SPLIT.
+    rewrite ! Any.pair_split. 
+    apply Any.split_pair. rewrite SPLIT. refl.
+
   - (* Tau *)
     erewrite ! (bisimulation_is_eq _ _ (translate_tau _ _)).
     rewrite ! interp_Es_tau.
     gstep. apply simg_tauL; et. apply simg_tauR; et. 
     apply simg_progress; et.
-    gfinal. left. eapply CIH'. ss.
+    gfinal. left. eapply CIH'. ss. et.
+    unfold assoc_ems. et.
+    (* exists x. et. *)
   - (* Vis *)
     erewrite ! (bisimulation_is_eq _ _ (translate_vis _ _ _ _)).
     destruct e0 as [c|[s|e0]].
     + (* call E *)
       rewrite <- ! bind_trigger, ! interp_Es_bind.
-      (* Set Printing All. *)
-      pattern (@interp_Es X (@prog (add (add ms0 ms1) ms2)) (@ITree.trigger Es X (@assoc_Es X (@inl1 callE (sum1 sE eventE) X c))) (assoc str)).
-      pattern (@interp_Es X (@prog (add ms0 (add ms1 ms2))) (@ITree.trigger Es X (@inl1 callE (sum1 sE eventE) X c)) str).
+      Set Printing All.
+      pattern (@interp_Es X (@prog (add (add ms0 ms1) ms2))
+      (@ITree.trigger Es X (@assoc_Es' X (@inl1 callE (sum1 sE eventE) X c))) 
+      (assoc' str)).
+      pattern (@interp_Es X (@prog (add ms0 (add ms1 ms2)))
+      (@ITree.trigger Es X (@inl1 callE (sum1 sE eventE) X c)) str).
       setoid_rewrite interp_Es_callE.
       setoid_rewrite interp_Es_callE.
       rewrite ! bind_tau.
@@ -605,28 +1775,60 @@ Proof. Admitted.
       apply simg_progress; et.
       rewrite <- ! interp_Es_bind.
     
-      gfinal. left. eapply CIH'.
-      unfold assoc_ems. erewrite ! (bisimulation_is_eq _ _ (translate_bind _ _ _)).
-      f_equal. apply assoc_ems_prog.
+      gfinal. left. eapply CIH'. et.
+      ss. unfold assoc_ems.
+      erewrite ! (bisimulation_is_eq _ _ (translate_bind _ _ _)).
+      f_equal.
+      (* admit. *)
+       apply assoc_ems_prog.
     + (* sE *)
       rewrite <- ! bind_trigger, ! interp_Es_bind.
-      (* Set Printing All. *)
-      pattern (@interp_Es X (@prog (add (add ms0 ms1) ms2)) (@ITree.trigger Es X (@assoc_Es X (@inr1 callE (sum1 sE eventE) X (@inl1 sE eventE X s)))) (assoc str)).
-      pattern (@interp_Es X (@prog (add ms0 (add ms1 ms2))) (@ITree.trigger Es X (@inr1 callE (sum1 sE eventE) X (@inl1 sE eventE X s))) str).
+      Set Printing All.
+      pattern (@interp_Es X (@prog (add (add ms0 ms1) ms2))
+      (@ITree.trigger Es X (@assoc_Es' X (@inr1 callE (sum1 sE eventE) X (@inl1 sE eventE X s))))
+      (assoc' str)). 
+      pattern (@interp_Es X (@prog (add ms0 (add ms1 ms2)))
+      (@ITree.trigger Es X (@inr1 callE (sum1 sE eventE) X (@inl1 sE eventE X s))) str).
       setoid_rewrite interp_Es_sE.
       grind.
-      (* Set Printing All. *)
-      pattern (@interp_Es X (@prog (add (add ms0 ms1) ms2))
-      (@ITree.trigger Es X (@inr1 callE (sum1 sE eventE) X (@inl1 sE eventE X (@SUpdate X (@assoc_state X run))))) (assoc str)).
       setoid_rewrite interp_Es_sE.
       grind.
       gstep. 
       apply simg_tauL; et. apply simg_tauR; et.
       apply simg_tauL; et. apply simg_tauR; et.
       apply simg_progress; et.
-      unfold assoc_state in *. 
+      unfold assoc_state, assoc' in Heq0.
+      rewrite SPLIT in Heq0.
+      rewrite ! Any.pair_split in Heq0.
+      hexploit SPLIT. i. apply Any.split_pair in H. des.
+      rewrite H in Heq.
+      rewrite Heq in Heq0.
+      replace t1 with (assoc' t0).
+      2: { inv Heq0. unfold assoc'. et. }
+      gfinal. left.
+      destruct (Any.split t0) eqn: T0.
+      * destruct p. s. destruct (Any.split t3) eqn: T3.
+        -- destruct p. s. apply Any.split_pair in T0, T3.
+           des. clarify. 
+           eapply CIH'.
+           ++ rewrite Any.pair_split. et.
+           ++ unfold assoc_ems. et.
+        -- clarify. eapply CIH'.  
+
+      inv Heq0. 
+      destruct (Any.split t0) eqn:T0.
+      * destruct p. s.
+        destruct (Any.split t2) eqn:T2.
+        -- destruct p. s.
+           apply Any.split_pair in T0, T2. des. clarify.
+           gfinal. left. apply CIH'.
+
+
+      (* Do we have that 'SUpdate run' maintains the pairing status of Any.t? *)
+      (* Either "pair-invariant" exists or some good associativity definition for non-splittable Any.t *)
+
       (* make lemma of assoc_assoc *)
-      assert (assoc_assoc: forall x, assoc' (assoc x) = x). 
+      (* assert (assoc_assoc: forall x, assoc' (assoc x) = x). 
       { i. unfold assoc, assoc'. des_ifs.
         - rewrite Any.pair_split in Heq1.
           inv Heq1. inv Heq4. 
@@ -635,27 +1837,17 @@ Proof. Admitted.
           rewrite Heq3. f_equal. f_equal.
           rewrite <- Any.split_pair with (a:=t7); et.
         all: admit.
-      }
+      } *)
       admit.
-      (* rewrite assoc_assoc in Heq0.
-      destruct str. destruct s4. inv Heq1.
-      (* rewrite H0 in Heq. *)
-      assert (SSS: (s, x) = (s1, (s0, s3), x0)). { rewrite <- H0, <- Heq. et. }
-      inv SSS.
-      gfinal. left.
-      replace (s1, s0, s3) with (assoc (s1, (s0, s3))); et.
-      eapply CIH'. unfold assoc_ems. et. *)
   + (* eventE *)
-    rewrite <- ! bind_trigger, ! interp_Es_bind. admit.
+    rewrite <- ! bind_trigger, ! interp_Es_bind.
     (* Set Printing All. *)
-    pattern (@interp_Es (prod (prod (state ms0) (state ms1)) (state ms2)) X0 (@prog (add (add ms0 ms1) ms2))
-    (@ITree.trigger (Es (prod (prod (state ms0) (state ms1)) (state ms2))) X0
-       (@assoc_Es (state ms0) (state ms1) (state ms2) X0
-          (@inr1 callE (sum1 (sE (state (add ms0 (add ms1 ms2)))) eventE) X0 (@inr1 (sE (state (add ms0 (add ms1 ms2)))) eventE X0 e0))))
-    (@assoc (state ms0) (state ms1) (state ms2) str)).
-    pattern (@interp_Es (state (add ms0 (add ms1 ms2))) X0 (@prog (add ms0 (add ms1 ms2)))
-    (@ITree.trigger (Es (state (add ms0 (add ms1 ms2)))) X0
-       (@inr1 callE (sum1 (sE (state (add ms0 (add ms1 ms2)))) eventE) X0 (@inr1 (sE (state (add ms0 (add ms1 ms2)))) eventE X0 e0))) str).
+    pattern (@interp_Es X (@prog (add (add ms0 ms1) ms2))
+    (@ITree.trigger Es X (@assoc_Es' X (@inr1 callE (sum1 sE eventE) X (@inr1 sE eventE X e0))))
+    (assoc' (Any.pair st0 (Any.pair st1 st2)))).
+    pattern (@interp_Es X (@prog (add ms0 (add ms1 ms2)))
+    (@ITree.trigger Es X (@inr1 callE (sum1 sE eventE) X (@inr1 sE eventE X e0)))
+    (Any.pair st0 (Any.pair st1 st2))).
     setoid_rewrite interp_Es_eventE.
     setoid_rewrite interp_Es_eventE.
     grind.
@@ -683,7 +1875,7 @@ Proof. Admitted.
       apply simg_tauL; et. apply simg_tauR; et.
       apply simg_progress; et.
       gfinal. left. apply CIH'. unfold assoc_ems. et.
-Qed.  *)
+Qed. 
 
 Lemma add_assoc_rev_aux
         ms0 ms1 ms2
