proofmode/HTactics.v
@@ -5,7 +5,9 @@ Require Import ModSem.
 Require Import Skeleton.
 Require Import PCM.
 Require Import Any.
-Require Import HoareDef STB SimModSem.
+Require Import HoareDef.
+Require Import SimModSem.
+Require Import STB.
 
 Require Import Relation_Definitions.
 Require Import Relation_Operators.
@@ -13,7 +15,8 @@ Require Import RelationPairs.
 From ExtLib Require Import
      Data.Map.FMapAList.
 Require Import Red IRed.
-Require Import ProofMode Invariant.
+Require Import ProofMode.
+Require Import Invariant.
 
 Set Implicit Arguments.
 
@@ -67,94 +70,94 @@ Ltac ired_both := ired_l; ired_r.
 Section SIM.
   Variable world: Type.
 
-  (* Let st_local: Type := (Any.t). *)
-  (* Let W: Type := (Any.t) * (Any.t). *)
+  Let st_local: Type := (Any.t).
+  Let W: Type := (Any.t) * (Any.t).
 
-  (* Variable wf: world -> W -> Prop. *)
+  Variable wf: world -> W -> Prop.
   Variable le: relation world.
 
   Variant _safe_sim_itree
-          (r g: forall (st_src st_tgt R_src R_tgt: Type) (wf: world -> (st_src * st_tgt) -> Prop) (RR: st_src -> st_tgt -> R_src -> R_tgt -> Prop), bool -> bool -> world -> st_src * itree (Es st_src) R_src -> st_tgt * itree (Es st_tgt) R_tgt -> Prop)
-          {st_src st_tgt R_src R_tgt} (wf: world -> (st_src * st_tgt) -> Prop) (RR: st_src -> st_tgt -> R_src -> R_tgt -> Prop)
-    : bool -> bool -> world -> st_src * itree (Es st_src) R_src -> st_tgt * itree (Es st_tgt) R_tgt -> Prop :=
+          (r g: forall (R_src R_tgt: Type) (RR: st_local -> st_local -> R_src -> R_tgt -> Prop), bool -> bool -> world -> st_local * itree Es R_src -> st_local * itree Es R_tgt -> Prop)
+          {R_src R_tgt} (RR: st_local -> st_local -> R_src -> R_tgt -> Prop)
+    : bool -> bool -> world -> st_local * itree Es R_src -> st_local * itree Es R_tgt -> Prop :=
   | safe_sim_itree_ret
       i_src0 i_tgt0 w0 st_src0 st_tgt0
       v_src v_tgt
       (RET: RR st_src0 st_tgt0 v_src v_tgt)
     :
-      _safe_sim_itree r g wf RR i_src0 i_tgt0 w0 (st_src0, (Ret v_src)) (st_tgt0, (Ret v_tgt))
+      _safe_sim_itree r g RR i_src0 i_tgt0 w0 (st_src0, (Ret v_src)) (st_tgt0, (Ret v_tgt))
   | safe_sim_itree_call
       i_src0 i_tgt0 w st_src0 st_tgt0
       fn varg k_src k_tgt
       (SIM: exists w0,
           (<<WF: wf w0 (st_src0, st_tgt0)>>) /\
           (<<K: forall w1 vret st_src1 st_tgt1 (WLE: le w0 w1) (WF: wf w1 (st_src1, st_tgt1)),
-              g _ _ _ _ wf RR false false w (st_src1, k_src vret) (st_tgt1, k_tgt vret)>>))
+              g _ _ RR false false w (st_src1, k_src vret) (st_tgt1, k_tgt vret)>>))
     :
-      _safe_sim_itree r g wf RR i_src0 i_tgt0 w (st_src0, trigger (Call fn varg) >>= k_src)
+      _safe_sim_itree r g RR i_src0 i_tgt0 w (st_src0, trigger (Call fn varg) >>= k_src)
                       (st_tgt0, trigger (Call fn varg) >>= k_tgt)
   | safe_sim_itree_syscall
       i_src0 i_tgt0 w0 st_src0 st_tgt0
       fn varg rvs k_src k_tgt
       (K: forall vret,
-          g _ _ _ _ wf RR true true w0 (st_src0, k_src vret) (st_tgt0, k_tgt vret))
+          g _ _ RR true true w0 (st_src0, k_src vret) (st_tgt0, k_tgt vret))
     :
-      _safe_sim_itree r g wf RR i_src0 i_tgt0 w0 (st_src0, trigger (Syscall fn varg rvs) >>= k_src)
+      _safe_sim_itree r g RR i_src0 i_tgt0 w0 (st_src0, trigger (Syscall fn varg rvs) >>= k_src)
                       (st_tgt0, trigger (Syscall fn varg rvs) >>= k_tgt)
 
   | safe_sim_itree_tau_src
       i_src0 i_tgt0 w0 st_src0 st_tgt0
       i_src i_tgt
-      (K: r _ _ _ _ wf RR true i_tgt0 w0 (st_src0, i_src) (st_tgt0, i_tgt))
+      (K: r _ _ RR true i_tgt0 w0 (st_src0, i_src) (st_tgt0, i_tgt))
     :
-      _safe_sim_itree r g wf RR i_src0 i_tgt0 w0 (st_src0, tau;; i_src) (st_tgt0, i_tgt)
+      _safe_sim_itree r g RR i_src0 i_tgt0 w0 (st_src0, tau;; i_src) (st_tgt0, i_tgt)
 
   | safe_sim_itree_tau_tgt
       i_src0 i_tgt0 w0 st_src0 st_tgt0
       i_src i_tgt
-      (K: r _ _ _ _ wf RR i_src0 true w0 (st_src0, i_src) (st_tgt0, i_tgt))
+      (K: r _ _ RR i_src0 true w0 (st_src0, i_src) (st_tgt0, i_tgt))
     :
-      _safe_sim_itree r g wf RR i_src0 i_tgt0 w0 (st_src0, i_src) (st_tgt0, tau;; i_tgt)
+      _safe_sim_itree r g RR i_src0 i_tgt0 w0 (st_src0, i_src) (st_tgt0, tau;; i_tgt)
   | safe_sim_itree_choose_tgt
       i_src0 i_tgt0 w0 st_src0 st_tgt0
       X i_src k_tgt
-      (K: forall (x: X), r _ _ _ _ wf RR i_src0 true w0 (st_src0, i_src) (st_tgt0, k_tgt x))
+      (K: forall (x: X), r _ _ RR i_src0 true w0 (st_src0, i_src) (st_tgt0, k_tgt x))
     :
-      _safe_sim_itree r g wf RR i_src0 i_tgt0 w0 (st_src0, i_src)
+      _safe_sim_itree r g RR i_src0 i_tgt0 w0 (st_src0, i_src)
                       (st_tgt0, trigger (Choose X) >>= k_tgt)
                       
   | safe_sim_itree_take_src
       i_src0 i_tgt0 w0 st_src0 st_tgt0
       X k_src i_tgt
-      (K: forall (x: X), r _ _ _ _ wf RR true i_tgt0 w0 (st_src0, k_src x) (st_tgt0, i_tgt))
+      (K: forall (x: X), r _ _ RR true i_tgt0 w0 (st_src0, k_src x) (st_tgt0, i_tgt))
     :
-      _safe_sim_itree r g wf RR i_src0 i_tgt0 w0 (st_src0, trigger (Take X) >>= k_src)
+      _safe_sim_itree r g RR i_src0 i_tgt0 w0 (st_src0, trigger (Take X) >>= k_src)
                       (st_tgt0, i_tgt)
   
   | safe_sim_itree_supdate_src
     i_src0 i_tgt0 w0 st_src0 st_tgt0
     X k_src i_tgt
-    (run: st_src -> st_src * X)
-    (K: r _ _ _ _ wf RR true i_tgt0 w0 (fst (run st_src0), k_src (snd (run st_src0))) (st_tgt0, i_tgt))
+    (run: st_local -> st_local * X)
+    (K: r _ _ RR true i_tgt0 w0 (fst (run st_src0), k_src (snd (run st_src0))) (st_tgt0, i_tgt))
   :
-    _safe_sim_itree r g wf RR i_src0 i_tgt0 w0 (st_src0, trigger (SUpdate run) >>= k_src)
+    _safe_sim_itree r g RR i_src0 i_tgt0 w0 (st_src0, trigger (SUpdate run) >>= k_src)
                     (st_tgt0, i_tgt)
 
   | safe_sim_itree_supdate_tgt
     i_src0 i_tgt0 w0 st_src0 st_tgt0
     X i_src k_tgt
-    (run: st_tgt -> st_tgt * X)
-    (K: r _ _ _ _ wf RR i_src0 true w0 (st_src0, i_src) (fst (run st_tgt0), k_tgt (snd (run st_tgt0))))
+    (run: st_local -> st_local * X)
+    (K: r _ _ RR i_src0 true w0 (st_src0, i_src) (fst (run st_tgt0), k_tgt (snd (run st_tgt0))))
   :
-    _safe_sim_itree r g wf RR i_src0 i_tgt0 w0 (st_src0, i_src)
+    _safe_sim_itree r g RR i_src0 i_tgt0 w0 (st_src0, i_src)
                     (st_tgt0, trigger (SUpdate run) >>= k_tgt)
 
   .
 
   Lemma safe_sim_sim r g:
-    @_safe_sim_itree (gpaco11 (_sim_itree le) (cpn11 (_sim_itree le)) r g) (gpaco11 (_sim_itree le) (cpn11 (_sim_itree le)) g g)
-    <11=
-    gpaco11 (_sim_itree le) (cpn11 (_sim_itree le)) r g.
+    @_safe_sim_itree (gpaco8 (_sim_itree wf le) (cpn8 (_sim_itree wf le)) r g) (gpaco8 (_sim_itree wf le) (cpn8 (_sim_itree wf le)) g g)
+    <8=
+    gpaco8 (_sim_itree wf le) (cpn8 (_sim_itree wf le)) r g.
   Proof.
     i. eapply sim_itreeC_spec. inv PR; try by (econs; eauto).
     des. econs; eauto.
@@ -167,43 +170,43 @@ Section HLEMMAS.
   Context `{Σ: GRA.t}.
   Local Opaque GRA.to_URA.
 
-  Variant mk_wf (A: Type) {st_src st_tgt}
-          (R: A -> st_src -> st_tgt -> iProp)
-    : A -> st_src * Σ * st_tgt -> Prop :=
+  Variant mk_wf (A: Type) 
+          (R: A -> Any.t -> Any.t -> iProp)
+    : A -> Any.t * Any.t -> Prop :=
   | mk_wf_intro
       a
       mr_src mp_src mp_tgt
       (RSRC: URA.wf mr_src -> R a mp_src mp_tgt mr_src)
     :
-      mk_wf R a ((mp_src, mr_src), mp_tgt)
+      mk_wf R a ((Any.pair mp_src mr_src↑), mp_tgt)
   .
 
-  (* Definition inv_wf
+  Definition inv_wf
              `{@GRA.inG invRA Σ}
-             A {st_src st_tgt}
-             (R: A -> st_src -> st_tgt -> iProp)
-    : _ -> (st_src * Σ * st_tgt -> Prop) :=
+             A 
+             (R: A -> Any.t -> Any.t -> iProp)
+    : _ -> (Any.t *  Any.t -> Prop) :=
     @mk_wf
-      (A + st_src * st_tgt)%type
+      (A + Any.t * Any.t)%type
       (fun a' mp_src mp_tgt =>
          match a' with
          | inl a => R a mp_src mp_tgt
          | inr (mp_src1, mp_tgt1) => inv_closed ** ⌜mp_src1 = mp_src /\ mp_tgt1 = mp_tgt⌝
          end)%I
-  . *)
+  .
 
   Lemma hcall_clo_ord_weaken'
-        (fsp1: fspec) {st_src st_tgt}
+        (fsp1: fspec) 
         (x: shelve__ fsp1.(meta))
 
         A (a0: shelve__ A) FR
 
-        (le: A -> A -> Prop)  r rg a n m mr_src0 mp_src0
+        (le: A -> A -> Prop) r rg a n m mr_src0 mp_src0
         (fsp0: fspec)
         mp_tgt0 k_tgt k_src
         fn tbr ord_cur varg_src varg_tgt
-        (R: A -> st_src -> st_tgt -> iProp)
-        (eqr: (st_src * Σ) -> st_tgt -> Any.t -> Any.t -> Prop)
+        (R: A -> Any.t -> Any.t -> iProp)
+        (eqr: Any.t -> Any.t -> Any.t -> Any.t -> Prop)
 
         (WEAKER: fspec_weaker fsp1 fsp0)
 
@@ -216,17 +219,17 @@ Section HLEMMAS.
         (PURE: ord_lt (fsp1.(measure) x) ord_cur /\
                (tbr = true -> is_pure (fsp1.(measure) x)) /\ (tbr = false -> (fsp1.(measure) x) = ord_top))
 
-        (POST: forall (vret_tgt : Any.t) (mr_src1: Σ) (mp_src1: st_src) (mp_tgt1: st_tgt) a1
+        (POST: forall (vret_tgt : Any.t) (mr_src1: Σ) (mp_src1 mp_tgt1: Any.t) a1
                       (vret_src: Any.t)
                       (WLE: le a0 a1)
                       ctx1
                       (ACC: current_iProp ctx1 (FR ** R a1 mp_src1 mp_tgt1 ** fsp1.(postcond) x vret_src vret_tgt))
           ,
-                gpaco11 (_sim_itree le) (cpn11 (_sim_itree le)) rg rg _ _ _ _ (mk_wf R) eqr true false a
-                       ((mp_src1, mr_src1), k_src (ctx1, vret_src)) (mp_tgt1, k_tgt vret_tgt))
-    :
-      gpaco11 (_sim_itree le) (cpn11 (_sim_itree le)) r rg _ _ _ _ (mk_wf R) eqr m n a
-             ((mp_src0, mr_src0), (HoareCall _ tbr ord_cur fsp0 fn varg_src) ctx0 >>= k_src)
+                gpaco8 (_sim_itree (mk_wf R) le) (cpn8 (_sim_itree (mk_wf R) le)) rg rg _ _ eqr true false a
+                  (Any.pair mp_src1 mr_src1↑, k_src (ctx1, vret_src)) (mp_tgt1, k_tgt vret_tgt))
+                :
+      gpaco8 (_sim_itree (mk_wf R) le) (cpn8 (_sim_itree (mk_wf R) le)) r rg _ _ eqr m n a
+             (Any.pair mp_src0 mr_src0, (HoareCall tbr ord_cur fsp0 fn varg_src) ctx0 >>= k_src)
              (mp_tgt0, trigger (Call fn varg_tgt) >>= k_tgt)
   .
   Proof.
@@ -280,7 +283,7 @@ Section HLEMMAS.
 
   Lemma hcall_clo_ord_weaken
         Hns Rn Invn
-        (fsp1: fspec) {st_src st_tgt}
+        (fsp1: fspec) 
         (x: shelve__ fsp1.(meta))
 
         A (a0: shelve__ A)
@@ -289,8 +292,8 @@ Section HLEMMAS.
         (fsp0: fspec)
         mp_tgt0 k_tgt k_src
         fn tbr ord_cur varg_src varg_tgt
-        (R: A -> st_src -> st_tgt -> iProp)
-        (eqr: (st_src * Σ) -> st_tgt -> Any.t -> Any.t -> Prop)
+        (R: A -> Any.t -> Any.t -> iProp)
+        (eqr: Any.t -> Any.t -> Any.t -> Any.t -> Prop)
 
         (WEAKER: fspec_weaker fsp1 fsp0)
 
@@ -309,11 +312,11 @@ Section HLEMMAS.
                       ctx1
                       (ACC: current_iPropL ctx1 ((Invn, R a1 mp_src1 mp_tgt1) :: (Rn, fsp1.(postcond) x vret_src vret_tgt) :: snd (alist_pops Hns l)))
           ,
-            gpaco11 (_sim_itree le) (cpn11 (_sim_itree le)) rg rg _ _ _ _ (mk_wf R) eqr true false a
-                   ((mp_src1, mr_src1), k_src (ctx1, vret_src)) (mp_tgt1, k_tgt vret_tgt))
+            gpaco8 (_sim_itree (mk_wf R) le) (cpn8 (_sim_itree (mk_wf R) le)) rg rg _ _ eqr true false a
+                   ((Any.pair mp_src1 mr_src1↑), k_src (ctx1, vret_src)) (mp_tgt1, k_tgt vret_tgt))
     :
-      gpaco11 (_sim_itree le) (cpn11 (_sim_itree le)) r rg _ _ _ _ (mk_wf R) eqr m n a
-             ((mp_src0, mr_src0), (HoareCall _ tbr ord_cur fsp0 fn varg_src) ctx0 >>= k_src)
+      gpaco8 (_sim_itree (mk_wf R) le) (cpn8 (_sim_itree (mk_wf R) le)) r rg _ _ eqr m n a
+             ((Any.pair mp_src0 mr_src0), (HoareCall tbr ord_cur fsp0 fn varg_src) ctx0 >>= k_src)
              (mp_tgt0, trigger (Call fn varg_tgt) >>= k_tgt)
   .
   Proof.
@@ -331,7 +334,7 @@ Section HLEMMAS.
   Qed.
 
   Lemma hcall_clo_weaken
-        Hns Rn Invn {st_src st_tgt}
+        Hns Rn Invn 
         (fsp1: fspec)
         (x: shelve__ fsp1.(meta))
 
@@ -341,8 +344,8 @@ Section HLEMMAS.
         (fsp0: fspec)
         mp_tgt0 k_tgt k_src
         fn tbr ord_cur varg_src varg_tgt
-        (R: A -> st_src -> st_tgt -> iProp)
-        (eqr: (st_src * Σ) -> st_tgt -> Any.t -> Any.t -> Prop)
+        (R: A -> Any.t -> Any.t -> iProp)
+        (eqr: Any.t -> Any.t -> Any.t -> Any.t -> Prop)
 
         (WEAKER: fspec_weaker fsp1 fsp0)
 
@@ -361,11 +364,11 @@ Section HLEMMAS.
                       ctx1
                       (ACC: current_iPropL ctx1 (@cons (prod string (bi_car iProp)) (Invn, R a1 mp_src1 mp_tgt1) (@cons (prod string (bi_car iProp)) (Rn, fsp1.(postcond) x vret_src vret_tgt) (snd (alist_pops Hns l)))))
           ,
-            gpaco11 (_sim_itree le) (cpn11 (_sim_itree le)) rg rg _ _ _ _ (mk_wf R) eqr true false a
-                   ((mp_src1, mr_src1), k_src (ctx1, vret_src)) (mp_tgt1, k_tgt vret_tgt))
+            gpaco8 (_sim_itree (mk_wf R) le) (cpn8 (_sim_itree (mk_wf R) le)) rg rg _ _ eqr true false a
+                   ((Any.pair mp_src1 mr_src1↑), k_src (ctx1, vret_src)) (mp_tgt1, k_tgt vret_tgt))
     :
-      gpaco11 (_sim_itree le) (cpn11 (_sim_itree le)) r rg _ _ _ _ (mk_wf R) eqr m n a
-             ((mp_src0, mr_src0), (HoareCall _ tbr ord_cur fsp0 fn varg_src) ctx0 >>= k_src)
+      gpaco8 (_sim_itree (mk_wf R) le) (cpn8 (_sim_itree (mk_wf R) le)) r rg _ _ eqr m n a
+             ((Any.pair mp_src0 mr_src0), (HoareCall tbr ord_cur fsp0 fn varg_src) ctx0 >>= k_src)
              (mp_tgt0, trigger (Call fn varg_tgt) >>= k_tgt)
   .
   Proof.
@@ -376,15 +379,15 @@ Section HLEMMAS.
         Hns Rn Invn
         X (x: shelve__ X)
         A (a0: shelve__ A)
-        {st_src st_tgt}
+        
         (D: X -> ord)
         (P: X -> Any.t -> Any.t -> iProp)
         (Q: X -> Any.t -> Any.t -> iProp)
         (le: A -> A -> Prop)  r rg a n m mr_src0 mp_src0
         mp_tgt0 k_tgt k_src
         fn tbr ord_cur varg_src varg_tgt
-        (R: A -> st_src -> st_tgt -> iProp)
-        (eqr: (st_src * Σ) -> st_tgt -> Any.t -> Any.t -> Prop)
+        (R: A -> Any.t -> Any.t -> iProp)
+        (eqr: Any.t -> Any.t -> Any.t -> Any.t -> Prop)
 
         ctx0 l
         (ACC: current_iPropL ctx0 l)
@@ -401,11 +404,11 @@ Section HLEMMAS.
                       ctx1
                       (ACC: current_iPropL ctx1 (@cons (prod string (bi_car iProp)) (Invn, R a1 mp_src1 mp_tgt1) (@cons (prod string (bi_car iProp)) (Rn, Q x vret_src vret_tgt) (snd (alist_pops Hns l)))))
           ,
-                gpaco11 (_sim_itree le) (cpn11 (_sim_itree le)) rg rg _ _ _ _ (mk_wf R) eqr true false a
-                       ((mp_src1, mr_src1), k_src (ctx1, vret_src)) (mp_tgt1, k_tgt vret_tgt))
+                gpaco8 (_sim_itree (mk_wf R) le) (cpn8 (_sim_itree (mk_wf R) le)) rg rg _ _ eqr true false a
+                       ((Any.pair mp_src1 mr_src1↑), k_src (ctx1, vret_src)) (mp_tgt1, k_tgt vret_tgt))
     :
-      gpaco11 (_sim_itree le) (cpn11 (_sim_itree le)) r rg _ _ _ _ (mk_wf R) eqr m n a
-             ((mp_src0, mr_src0), (HoareCall _ tbr ord_cur (mk_fspec D P Q) fn varg_src) ctx0 >>= k_src)
+      gpaco8 (_sim_itree (mk_wf R) le) (cpn8 (_sim_itree (mk_wf R) le)) r rg _ _ eqr m n a
+             ((Any.pair mp_src0 mr_src0), (HoareCall tbr ord_cur (mk_fspec D P Q) fn varg_src) ctx0 >>= k_src)
              (mp_tgt0, trigger (Call fn varg_tgt) >>= k_tgt)
   .
   Proof.
@@ -417,25 +420,25 @@ Section HLEMMAS.
   Qed.
 
   Lemma harg_clo
-        A Rn Invn {st_src st_tgt}
+        A Rn Invn 
          r rg
         X (P: X -> Any.t -> Any.t -> iProp) varg
         mpr_src mp_tgt f_tgt k_src
         a (le: A -> A -> Prop)
-        (R: A -> st_src -> st_tgt -> iProp)
-        (eqr: (st_src * Σ) -> st_tgt -> Any.t -> Any.t -> Prop)
+        (R: A -> Any.t -> Any.t -> iProp)
+        (eqr: Any.t -> Any.t -> Any.t -> Any.t -> Prop)
         (WF: mk_wf R a (mpr_src, mp_tgt))
         m n
         (ARG:
            forall x varg_src
                   ctx (mr_src: Σ) mp_src
                   (ACC: current_iPropL ctx (@cons (prod string (bi_car iProp)) (Rn, P  x varg_src varg) (@cons (prod string (bi_car iProp)) (Invn, R a mp_src mp_tgt) (@nil (prod string (bi_car iProp)))))),
-             gpaco11 (_sim_itree le) (cpn11 (_sim_itree le)) r rg _ _ _ _ (mk_wf R) eqr true n a
-                    ((mp_src, mr_src), k_src (ctx, (x, varg_src)))
+             gpaco8 (_sim_itree (mk_wf R) le) (cpn8 (_sim_itree (mk_wf R) le)) r rg _ _  eqr true n a
+                    ((Any.pair mp_src mr_src↑), k_src (ctx, (x, varg_src)))
                     (mp_tgt, f_tgt))
     :
-      gpaco11 (_sim_itree le) (cpn11 (_sim_itree le)) r rg _ _ _ _ (mk_wf R) eqr m n a
-             (mpr_src, (HoareFunArg _ P varg >>= k_src))
+      gpaco8 (_sim_itree (mk_wf R) le) (cpn8 (_sim_itree (mk_wf R) le)) r rg _ _  eqr m n a
+             (mpr_src, (HoareFunArg P varg >>= k_src))
              (mp_tgt, f_tgt)
   .
   Proof.
@@ -458,14 +461,14 @@ Section HLEMMAS.
   Qed.
 
   Lemma hret_clo
-        A (a: shelve__ A) {st_src st_tgt}
+        A (a: shelve__ A) 
          r rg n m mr_src mp_src a0
         X (Q: X -> Any.t -> Any.t -> iProp)
         x vret_src vret_tgt
         mp_tgt
         (le: A -> A -> Prop)
-        (eqr: (st_src * Σ) -> st_tgt -> Any.t -> Any.t -> Prop)
-        (R: A -> st_src -> st_tgt -> iProp)
+        (eqr: Any.t -> Any.t -> Any.t -> Any.t -> Prop)
+        (R: A -> Any.t -> Any.t -> iProp)
 
         ctx l
         (ACC: current_iPropL ctx l)
@@ -475,11 +478,11 @@ Section HLEMMAS.
         (UPDATABLE:
            (from_iPropL l) ⊢ #=> (R a mp_src mp_tgt ** (Q  x vret_src vret_tgt: iProp)))
 
-        (EQ: forall (mr_src1: Σ) (WLE: le a0 a) (WF: mk_wf R a ((mp_src, mr_src1), mp_tgt)),
-            eqr ((mp_src, mr_src1)) mp_tgt vret_tgt vret_tgt)
+        (EQ: forall (mr_src1: Σ) (WLE: le a0 a) (WF: mk_wf R a ((Any.pair mp_src mr_src1↑), mp_tgt)),
+            eqr ((Any.pair mp_src mr_src1↑)) mp_tgt vret_tgt vret_tgt)
     :
-      gpaco11 (_sim_itree le) (cpn11 (_sim_itree le)) r rg _ _ _ _ (mk_wf R) eqr m n a0
-             ((mp_src, mr_src), (HoareFunRet _ Q  x (ctx, vret_src)))
+      gpaco8 (_sim_itree (mk_wf R) le) (cpn8 (_sim_itree (mk_wf R) le)) r rg _ _  eqr m n a0
+             ((Any.pair mp_src mr_src), (HoareFunRet Q x (ctx, vret_src)))
              (mp_tgt, (Ret vret_tgt))
   .
   Proof.
@@ -506,23 +509,23 @@ Section HLEMMAS.
   Qed.
 
   Lemma APC_start_clo
-        (at_most: Ord.t) {st_src st_tgt}
+        (at_most: Ord.t) 
         (o: ord)
         A  r rg a m n mp_src0
         k_src
-        (wf: A -> st_src * Σ * st_tgt -> Prop)
+        (wf: A -> Any.t * Any.t -> Prop)
         (le: A -> A -> Prop)
-        (eqr: st_src * Σ -> st_tgt -> Any.t -> Any.t -> Prop)
+        (eqr: Any.t -> Any.t -> Any.t -> Any.t -> Prop)
         stb itr_tgt ctx
 
-        (POST: gpaco11 (_sim_itree le) (cpn11 (_sim_itree le)) r rg _ _ _ _ wf eqr true n a
+        (POST: gpaco8 (_sim_itree wf le) (cpn8 (_sim_itree wf le)) r rg _ _ eqr true n a
                       (mp_src0,
-                       (interp_hCallE_tgt  stb o (_APC _ at_most) ctx)>>= k_src)
+                       (interp_hCallE_tgt  stb o (_APC at_most) ctx)>>= k_src)
                       (itr_tgt))
     :
-      gpaco11 (_sim_itree le) (cpn11 (_sim_itree le)) r rg _ _ _ _ wf eqr m n a
+      gpaco8 (_sim_itree wf le) (cpn8 (_sim_itree wf le)) r rg _ _ eqr m n a
              (mp_src0,
-              (interp_hCallE_tgt stb o (APC _) ctx) >>= k_src)
+              (interp_hCallE_tgt stb o APC ctx) >>= k_src)
              (itr_tgt).
   Proof. 
     subst.  unfold APC. destruct itr_tgt. ired_both.
@@ -538,26 +541,26 @@ Section HLEMMAS.
     exists at_most.
     repeat (ired_both; apply sim_itreeC_spec; econs).
     ired_both. et.
-    Unshelve. all: ss.
+    (* Unshelve. all: ss. *)
   Qed.
 
   Lemma APC_stop_clo
-        (o: ord) {st_src st_tgt}
+        (o: ord) 
         A  r rg a n m mp_src0
         k_src
         (at_most: Ord.t)
-        (wf: A -> st_src * Σ * st_tgt -> Prop)
+        (wf: A -> Any.t * Any.t -> Prop)
         (le: A -> A -> Prop)
-        (eqr: (st_src * Σ) -> st_tgt -> Any.t -> Any.t -> Prop)
+        (eqr: Any.t -> Any.t -> Any.t -> Any.t -> Prop)
         stb itr_tgt ctx
 
-        (POST: gpaco11 (_sim_itree le) (cpn11 (_sim_itree le)) r rg _ _ _ _ wf eqr true n a
+        (POST: gpaco8 (_sim_itree wf le) (cpn8 (_sim_itree wf le)) r rg _ _ eqr true n a
                       (mp_src0, k_src (ctx, ()))
                       (itr_tgt))
     :
-      gpaco11 (_sim_itree le) (cpn11 (_sim_itree le)) r rg _ _ _ _ wf eqr m n a
+      gpaco8 (_sim_itree wf le) (cpn8 (_sim_itree wf le)) r rg _ _ eqr m n a
               (mp_src0,
-              (interp_hCallE_tgt  stb o (_APC _ at_most) ctx) >>= k_src)
+              (interp_hCallE_tgt  stb o (_APC at_most) ctx) >>= k_src)
              (itr_tgt).
   Proof. 
     subst. destruct itr_tgt.
@@ -571,28 +574,28 @@ Section HLEMMAS.
 
   Lemma APC_step_clo
         (fn: gname) (args: Any.t) (next: Ord.t)
-        {st_src st_tgt}
+        
         (o: ord)
         A  r rg a n m mp_src0
         k_src ctx0
         (at_most: Ord.t)
-        (wf: A -> st_src * Σ * st_tgt -> Prop)
+        (wf: A -> Any.t * Any.t -> Prop)
         (le: A -> A -> Prop)
-        (eqr: (st_src * Σ) -> st_tgt -> Any.t -> Any.t -> Prop)
+        (eqr: Any.t -> Any.t -> Any.t -> Any.t -> Prop)
         stb itr_tgt
 
         (fsp: fspec)
         (FIND: stb fn = Some fsp)
         (NEXT: (next < at_most)%ord)
 
-        (POST: gpaco11 (_sim_itree le) (cpn11 (_sim_itree le)) r rg _ _ _ _ wf eqr true n a
+        (POST: gpaco8 (_sim_itree wf le) (cpn8 (_sim_itree wf le)) r rg _ _ eqr true n a
                       (mp_src0,
-                       ('(ctx1, _) <- (HoareCall _ true o fsp fn args ctx0);;
-                        Tau (ITree.bind (interp_hCallE_tgt  stb o (_APC _ next) ctx1) k_src)))
+                       ('(ctx1, _) <- (HoareCall true o fsp fn args ctx0);;
+                        Tau (ITree.bind (interp_hCallE_tgt  stb o (_APC next) ctx1) k_src)))
                       (itr_tgt))
     :
-      gpaco11 (_sim_itree le) (cpn11 (_sim_itree le)) r rg _ _ _ _ wf eqr m n a
-             (mp_src0, (interp_hCallE_tgt  stb o (_APC _ at_most) ctx0) >>= k_src)
+      gpaco8 (_sim_itree wf le) (cpn8 (_sim_itree wf le)) r rg _ _ eqr m n a
+             (mp_src0, (interp_hCallE_tgt  stb o (_APC at_most) ctx0) >>= k_src)
              (itr_tgt).
   Proof. 
     subst. destruct itr_tgt.
@@ -619,7 +622,7 @@ Section HLEMMAS.
     (* rewrite interp_tgt_bind. rewrite interp_tgt_hcall. rewrite bind_bind. rewrite bind_bind. *)
     ss. rewrite FIND. ss. subst. ired_l.
     match goal with
-    | [SIM: gpaco11 _ _ _ _ _ _ _ _ _ _ _ _ _ ?i0 _ |- gpaco11 _ _ _ _ _ _ _ _ _ _ _ _ _ ?i1 _] =>
+    | [SIM: gpaco8 _ _ _ _ _ _ _ _ _ _ ?i0 _ |- gpaco8 _ _ _ _ _ _ _ _ _ _ ?i1 _] =>
       replace i1 with i0; et
     end.
     f_equal. grind.
@@ -629,12 +632,12 @@ Section HLEMMAS.
         A wf (le: A -> A -> Prop) r rg w arg mrp_src mp_tgt itr_tgt  stb body RR
         m n
         (INIT:
-           gpaco11 (_sim_itree wf le) (cpn11 (_sim_itree wf le)) r rg Any.t Any.t
+           gpaco8 (_sim_itree wf le) (cpn8 (_sim_itree wf le)) r rg Any.t Any.t
                   RR true n w
                   (mrp_src, fun_to_tgt  stb (mk_specbody fspec_trivial body) arg)
                   (mp_tgt, itr_tgt))
     :
-      gpaco11 (_sim_itree wf le) (cpn11 (_sim_itree wf le)) r rg Any.t Any.t
+      gpaco8 (_sim_itree wf le) (cpn8 (_sim_itree wf le)) r rg Any.t Any.t
              RR m n w
              (mrp_src, KModSem.disclose_ksb_tgt  stb (ksb_trivial body) arg)
              (mp_tgt, itr_tgt).
@@ -651,20 +654,20 @@ Ltac prep := ired_both.
 Ltac _force_l :=
   prep;
   match goal with
-  | [ |- (gpaco11 (_sim_itree _) _ _ _ _ _ _ _ _ _ _ _ _ (_, unwrapN ?ox >>= _) (_, _)) ] =>
+  | [ |- (gpaco8 (_sim_itree _ _) _ _ _ _ _ _ _ _ _ (_, unwrapN ?ox >>= _) (_, _)) ] =>
     let tvar := fresh "tmp" in
     let thyp := fresh "TMP" in
     remember (unwrapN ox) as tvar eqn:thyp; unfold unwrapN in thyp; subst tvar;
     let name := fresh "_UNWRAPN" in
     destruct (ox) eqn:name; [|exfalso]; cycle 1
-  | [ |- (gpaco11 (_sim_itree _) _ _ _ _ _ _ _ _ _ _ _ _ (_, guarantee ?P >>= _) (_, _)) ] =>
+  | [ |- (gpaco8 (_sim_itree _ _) _ _ _ _ _ _ _ _ _ (_, guarantee ?P >>= _) (_, _)) ] =>
     let tvar := fresh "tmp" in
     let thyp := fresh "TMP" in
     remember (guarantee P) as tvar eqn:thyp; unfold guarantee in thyp; subst tvar;
     let name := fresh "_GUARANTEE" in
     destruct (classic P) as [name|name]; [ired_both; apply sim_itreeC_spec; eapply sim_itreeC_choose_src; [exists name]|contradict name]; cycle 1
 
-  | [ |- (gpaco11 (_sim_itree _) _ _ _ _ _ _ _ _ _ _ _ _ (_, ITree.bind (interp _ guarantee ?P) _ (_, _))) ] =>
+  | [ |- (gpaco8 (_sim_itree _ _) _ _ _ _ _ _ _ _ _ (_, ITree.bind (interp _ guarantee ?P) _ (_, _))) ] =>
     let tvar := fresh "tmp" in
     let thyp := fresh "TMP" in
     remember (guarantee P) as tvar eqn:thyp; unfold guarantee in thyp; subst tvar;
@@ -672,14 +675,14 @@ Ltac _force_l :=
     destruct (classic P) as [name|name]; [ired_both; apply sim_itreeC_spec; eapply sim_itreeC_choose_src; [exists name]|contradict name]; cycle 1
 
    (* TODO: handle interp_hCallE_tgt better and remove this case *)
-  | [ |- (gpaco11 (_sim_itree _) _ _ _ _ _ _ _ _ _ _ _ _ (_, ITree.bind (interp _ (guarantee ?P )) _) (_, _)) ] =>
+  | [ |- (gpaco8 (_sim_itree _ _) _ _ _ _ _ _ _ _ _ (_, ITree.bind (interp _ (guarantee ?P )) _) (_, _)) ] =>
     let tvar := fresh "tmp" in
     let thyp := fresh "TMP" in
     remember (guarantee P) as tvar eqn:thyp; unfold guarantee in thyp; subst tvar;
     let name := fresh "_GUARANTEE" in
     destruct (classic P) as [name|name]; [ired_both; apply sim_itreeC_spec; eapply sim_itreeC_choose_src; [exists name]|contradict name]; cycle 1; clear name
 
-  | [ |- (gpaco11 (_sim_itree _) _ _ _ _ _ _ _ _ _ _ _ _ (_, ?i_src) (_, ?i_tgt)) ] =>
+  | [ |- (gpaco8 (_sim_itree _ _) _ _ _ _ _ _ _ _ _ (_, ?i_src) (_, ?i_tgt)) ] =>
     seal i_tgt; apply sim_itreeC_spec; econs; unseal i_tgt
   end
 .
@@ -687,20 +690,20 @@ Ltac _force_l :=
 Ltac _force_r :=
   prep;
   match goal with
-  | [ |- (gpaco11 (_sim_itree _) _ _ _ _ _ _ _ _ _ _ _ _ (_, _) (_, unwrapU ?ox >>= _)) ] =>
+  | [ |- (gpaco8 (_sim_itree _ _) _ _ _ _ _ _ _ _ _ (_, _) (_, unwrapU ?ox >>= _)) ] =>
     let tvar := fresh "tmp" in
     let thyp := fresh "TMP" in
     remember (unwrapU ox) as tvar eqn:thyp; unfold unwrapU in thyp; subst tvar;
     let name := fresh "_UNWRAPU" in
     destruct (ox) eqn:name; [|exfalso]; cycle 1
-  | [ |- (gpaco11 (_sim_itree _) _ _ _ _ _ _ _ _ _ _ _ _ (_, _) (_, assume ?P >>= _)) ] =>
+  | [ |- (gpaco8 (_sim_itree _ _) _ _ _ _ _ _ _ _ _ (_, _) (_, assume ?P >>= _)) ] =>
     let tvar := fresh "tmp" in
     let thyp := fresh "TMP" in
     remember (assume P) as tvar eqn:thyp; unfold assume in thyp; subst tvar;
     let name := fresh "_ASSUME" in
     destruct (classic P) as [name|name]; [ired_both; apply sim_itreeC_spec; eapply sim_itreeC_take_tgt; [exists name]|contradict name]; cycle 1
 
-  | [ |- (gpaco11 (_sim_itree _) _ _ _ _ _ _ _ _ _ _ _ _ (_, ?i_src) (_, ?i_tgt)) ] =>
+  | [ |- (gpaco8 (_sim_itree _ _) _ _ _ _ _ _ _ _ _ (_, ?i_src) (_, ?i_tgt)) ] =>
     seal i_src; apply sim_itreeC_spec; econs; unseal i_src
   end
 .
@@ -709,15 +712,15 @@ Ltac _step :=
   match goal with
   (*** blacklisting ***)
   (* | [ |- (gpaco5 (_sim_itree wf) _ _ _ _ (_, trigger (Choose _) >>= _) (_, ?i_tgt)) ] => idtac *)
-  | [ |- (gpaco11 (_sim_itree _) _ _ _ _ _ _ _ _ _ _ _ _ (_, triggerUB >>= _) (_, _)) ] =>
+  | [ |- (gpaco8 (_sim_itree _ _) _ _ _ _ _ _ _ _ _ (_, triggerUB >>= _) (_, _)) ] =>
     unfold triggerUB; ired_l; _step; done
-  | [ |- (gpaco11 (_sim_itree _) _ _ _ _ _ _ _ _ _ _ _ _ (_, unwrapU ?ox >>= _) (_, _)) ] =>
+  | [ |- (gpaco8 (_sim_itree _ _) _ _ _ _ _ _ _ _ _ (_, unwrapU ?ox >>= _) (_, _)) ] =>
     let tvar := fresh "tmp" in
     let thyp := fresh "TMP" in
     remember (unwrapU ox) as tvar eqn:thyp; unfold unwrapU in thyp; subst tvar;
     let name := fresh "_UNWRAPU" in
     destruct (ox) eqn:name; [|unfold triggerUB; ired_both; _force_l; ss; fail]
-  | [ |- (gpaco11 (_sim_itree _) _ _ _ _ _ _ _ _ _ _ _ _ (_, assume ?P >>= _) (_, _)) ] =>
+  | [ |- (gpaco8 (_sim_itree _ _) _ _ _ _ _ _ _ _ _ (_, assume ?P >>= _) (_, _)) ] =>
     let tvar := fresh "tmp" in
     let thyp := fresh "TMP" in
     remember (assume P) as tvar eqn:thyp; unfold assume in thyp; subst tvar;
@@ -726,15 +729,15 @@ Ltac _step :=
 
   (*** blacklisting ***)
   (* | [ |- (gpaco5 (_sim_itree wf) _ _ _ _ (_, _) (_, trigger (Take _) >>= _)) ] => idtac *)
-  | [ |- (gpaco11 (_sim_itree _) _ _ _ _ _ _ _ _ _ _ _ _ (_, triggerNB >>= _) (_, _)) ] =>
+  | [ |- (gpaco8 (_sim_itree _ _) _ _ _ _ _ _ _ _ _ (_, triggerNB >>= _) (_, _)) ] =>
     unfold triggerNB; ired_r; _step; done
-  | [ |- (gpaco11 (_sim_itree _) _ _ _ _ _ _ _ _ _ _ _ _ (_, _) (_, unwrapN ?ox >>= _)) ] =>
+  | [ |- (gpaco8 (_sim_itree _ _) _ _ _ _ _ _ _ _ _ (_, _) (_, unwrapN ?ox >>= _)) ] =>
     let tvar := fresh "tmp" in
     let thyp := fresh "TMP" in
     remember (unwrapN ox) as tvar eqn:thyp; unfold unwrapN in thyp; subst tvar;
     let name := fresh "_UNWRAPN" in
     destruct (ox) eqn:name; [|unfold triggerNB; ired_both; _force_r; ss; fail]
-  | [ |- (gpaco11 (_sim_itree _) _ _ _ _ _ _ _ _ _ _ _ _ (_, _) (_, guarantee ?P >>= _)) ] =>
+  | [ |- (gpaco8 (_sim_itree _ _) _ _ _ _ _ _ _ _ _ (_, _) (_, guarantee ?P >>= _)) ] =>
     let tvar := fresh "tmp" in
     let thyp := fresh "TMP" in
     remember (guarantee P) as tvar eqn:thyp; unfold guarantee in thyp; subst tvar;
@@ -752,6 +755,7 @@ Ltac _step :=
   | _ => idtac
   end
 .
+
 Ltac _steps := repeat ((*** pre processing ***) prep; try _step; (*** post processing ***) simpl).
 
 Ltac steps := repeat ((*** pre processing ***) prep; try _step; (*** post processing ***) simpl; des_ifs_safe).
@@ -760,13 +764,13 @@ Ltac force_r := _force_r.
 
 Notation "wf n '------------------------------------------------------------------' src0 tgt0 '------------------------------------------------------------------' src1 '------------------------------------------------------------------' src2 tgt2"
   :=
-    (gpaco11 (_sim_itree _) _ _ _ _ _ _ _ wf _ _ _ n ((src0, src1), src2) (tgt0, tgt2))
+    (gpaco8 (_sim_itree wf _) _ _ _ _ _ _ _ _ n ((Any.pair src0 src1), src2) (tgt0, tgt2))
       (at level 60,
        format "wf  n '//' '------------------------------------------------------------------' '//' src0 '//' tgt0 '//' '------------------------------------------------------------------' '//' src1 '//' '------------------------------------------------------------------' '//' src2 '//' '//' '//' tgt2 '//' ").
 
 Notation "wf n '------------------------------------------------------------------' src0 tgt0 '------------------------------------------------------------------' '------------------------------------------------------------------' src2 tgt2"
   :=
-    (gpaco11 (_sim_itree _) _ _ _ _ _ _ _ wf _ _ _ n (src0, src2) (tgt0, tgt2))
+    (gpaco8 (_sim_itree wf _) _ _ _ _ _ _ _ _ n (src0, src2) (tgt0, tgt2))
       (at level 60,
        format "wf  n '//' '------------------------------------------------------------------' '//' src0 '//' tgt0 '//' '------------------------------------------------------------------' '//' '//' '------------------------------------------------------------------' '//' src2 '//' '//' '//' tgt2 '//' ").
 
@@ -774,16 +778,16 @@ Section TEST.
   Context `{Σ: GRA.t}.
   Let wf := (mk_wf (fun (_ : unit) (_ _ : Any.t) => bi_pure True)).
   Let le := fun (_ _: unit) => True.
-  Variable srcs0: Any.t * Σ.
+  Variable srcs0: Any.t.
   Variable tgts0: Any.t.
 
-  Goal gpaco11 (_sim_itree le) (cpn11 (_sim_itree le)) bot11 bot11 _ _ Any.t Any.t wf (fun _ _ => eq) false false tt
+  Goal gpaco8 (_sim_itree wf le) (cpn8 (_sim_itree wf le)) bot8 bot8 Any.t Any.t (fun _ _ => eq) false false tt
        (srcs0, triggerUB >>= idK) (tgts0, triggerUB >>= idK).
   Proof.
     steps.
   Qed.
 
-  Goal gpaco11 (_sim_itree le) (cpn11 (_sim_itree le)) bot11 bot11 _ _ Any.t Any.t wf (fun _ _ => eq) false false tt
+  Goal gpaco8 (_sim_itree wf le) (cpn8 (_sim_itree wf le)) bot8 bot8 Any.t Any.t (fun _ _ => eq) false false tt
        (srcs0, triggerNB >>= idK) (tgts0, triggerNB >>= idK).
   Proof.
     steps.
@@ -806,7 +810,7 @@ Ltac astep _fn _args :=
 
 Ltac acatch :=
   match goal with
-  | [ |- (gpaco11 (_sim_itree _) _ _ _ _ _ _ _ _ _ _ _ _ (_, _) (_, trigger (Call ?fn ?args) >>= _)) ] =>
+  | [ |- (gpaco8 (_sim_itree _ _) _ _ _ _ _ _ _ _ _ (_, _) (_, trigger (Call ?fn ?args) >>= _)) ] =>
     astep fn args
   end.
 
@@ -816,7 +820,7 @@ Ltac astart _at_most :=
 
 Ltac astop :=
   match goal with
-  | [ |- (gpaco11 (_sim_itree _) _ _ _ _ _ _ _ _ _ _ _ _ (_, interp_hCallE_tgt _ _ _ APC _ >>= _) (_, _)) ] => astart 0
+  | [ |- (gpaco8 (_sim_itree _ _) _ _ _ _ _ _ _ _ _ (_, interp_hCallE_tgt _ _ _ APC _ >>= _) (_, _)) ] => astart 0
   | _ => idtac
   end;
   eapply APC_stop_clo.
@@ -829,21 +833,10 @@ Ltac init :=
   let mrp_src := fresh "mrp_src" in
   let mp_tgt := fresh "mp_tgt" in
   let WF := fresh "WF" in
-  split; ss; intros varg_src [mn varg] EQ w mrp_src mp_tgt WF;
+  split; ss; intros varg_src varg EQ w mrp_src mp_tgt WF;
   try subst varg_src; cbn; ginit;
   try (unfold fun_to_tgt, cfunN, cfunU; rewrite HoareFun_parse); simpl
-(*   match goal with
-  | |- gpaco11 _ _ _ _ _ _ _ _ _ _ (_, KModSem.disclose_ksb_tgt _ _ (ksb_trivial _) _) _ =>
-    eapply trivial_init_clo;
-    try (unfold fun_to_tgt, cfunN, cfunU, KModSem.disclose_ksb_tgt, fun_to_tgt);
-    rewrite HoareFun_parse; simpl
-  | |- gpaco11 _ _ _ _ _ _ _ _ _ _ (_, KModSem.disclose_ksb_tgt _ _ _ _) _ =>
-    try (unfold fun_to_tgt, cfunN, cfunU, KModSem.disclose_ksb_tgt, fun_to_tgt);
-    simpl;
-    apply sim_itreeC_spec; apply sim_itreeC_take_src; intros [];rewrite HoareFun_parse; simpl
-  | |- _ =>
-    try (unfold fun_to_tgt, cfunN, cfunU; rewrite HoareFun_parse); simpl 
-  end  *)
+
   .
 
 Ltac harg :=
@@ -898,7 +891,7 @@ Ltac iarg :=
   i;
   mDesSep PRE as CLOSED PRE;
   match goal with
-  | [ |- (gpaco11 _ _ _ _ _ _ _ _ _ _ _ _ ?w _ _)] =>
+  | [ |- (gpaco8 _ _ _ _ _ _ _ _ _ ?w _ _)] =>
     destruct w as [?|[?mp_src ?mp_tgt]]; simpl;
     [
         |mAssertPure False; ss; iDestruct "INV" as "[INV _]"; iApply (inv_closed_unique with "☃CLOSED INV")
@@ -966,7 +959,7 @@ Lemma intro_hide_mark: forall A (a: A), a = __hide_mark a. refl. Qed.
 
 Ltac hide_k :=
   match goal with
-  | [ |- (gpaco11 _ _ _ _ _ _ _ _ _ _ _ _ _ (_, ?isrc >>= ?ksrc) (_, ?itgt >>= ?ktgt)) ] =>
+  | [ |- (gpaco8 _ _ _ _ _ _ _ _ _ _ (_, ?isrc >>= ?ksrc) (_, ?itgt >>= ?ktgt)) ] =>
     erewrite intro_hide_mark with (a:=ksrc);
     erewrite intro_hide_mark with (a:=ktgt);
     let name0 := fresh "__KSRC__" in set (__hide_mark ksrc) as name0; move name0 at top;
@@ -982,9 +975,9 @@ Ltac unhide_k :=
 
 Ltac deflag :=
   match goal with
-  | [ |- (gpaco11 _ _ _ _ _ _ _ _ _ _ true true _ _ _) ] =>
+  | [ |- (gpaco8 _ _ _ _ _ _ _ true true _ _ _) ] =>
     eapply sim_itree_progress_flag
-  | [ |- (gpaco11 _ _ _ _ _ _ _ _ _ _ _ _ _ _ _) ] =>
+  | [ |- (gpaco8 _ _ _ _ _ _ _ _ _ _ _ _) ] =>
     eapply sim_itree_flag_down
   | _ => fail
   end.
